hilbert2nj.v
@@ -4,52 +4,7 @@ Require Import stdlib_more.
 Require Export nj1 hilbert.
 
 
-Section H2N.
-
-Context { vatom : DecType } { tatom : Type } { fatom : Type }.
-Notation term := (@term vatom tatom).
-Notation closed t := (freevars t = nil).
-Notation tup := (@tup vatom tatom).
-Notation hterm := (@hterm vatom tatom).
-Notation hclosed t := (hfreevars t = nil).
-Notation formula := (@formula vatom tatom fatom).
-Notation hformula := (@hformula vatom tatom fatom).
-
-Hint Rewrite
-  (@tup_tup_com vatom tatom) (@tup_tsubs_com vatom tatom)
-  (@ntsubs_tup_com vatom tatom) (@ntsubs_z_tup vatom tatom)
-  (@freevars_tup vatom tatom) (@tsubs_tsubs_eq vatom tatom) : term_db.
-Hint Resolve (@closed_nofreevars vatom tatom) : term_db.
-Hint Rewrite (@freevars_ntsubs vatom tatom) using intuition; fail : term_db.
-Hint Rewrite (@nfree_tsubs vatom tatom)
-  using try (intuition; fail); (try apply closed_nofreevars); intuition; fail : term_db.
-Hint Rewrite (@ntsubs_tsubs_com vatom tatom)
-  using try (intuition; fail); (try apply closed_nofreevars); intuition; fail : term_db.
-Hint Rewrite (@tsubs_tsubs_com vatom tatom)
-  using try (intuition; fail); (try apply closed_nofreevars); intuition; fail : term_db.
-Hint Rewrite (@freevars_tsubs_closed vatom tatom)
-  using intuition; fail : term_db.
-
-Ltac formula_induction A :=
-  (try intros until A) ;
-  let XX := fresh "X" in
-  let xx := fresh "x" in
-  let A1 := fresh A in
-  let A2 := fresh A in
-  let ll := fresh "l" in
-  let lll := fresh "l" in
-  let tt := fresh "t" in
-  let IHll := fresh "IHl" in
-  induction A as [ XX ll | A1 ? A2 ? | xx A | xx A ]; simpl; intros;
-  [ rewrite ? flat_map_concat_map;
-    try f_equal; try (induction ll as [ | tt lll IHll ]; simpl; intuition;
-                      rewrite IHll; f_equal; intuition)
-  | try (f_equal; intuition)
-  | try (repeat case_analysis; intuition; f_equal; intuition; (rnow idtac); fail)
-  | try (repeat case_analysis; intuition; f_equal; intuition; (rnow idtac); fail) ];
-  try (now (rnow idtac)); try (now rcauto).
-
-Ltac hterm_induction t :=
+Ltac term_induction t :=
   (try intros until t);
   let nn := fresh "n" in
   let xx := fresh "x" in
@@ -58,15 +13,73 @@ Ltac hterm_induction t :=
   let IHll := fresh "IHl" in
   let i := fresh "i" in
   let Hi := fresh "Hi" in
-  apply (hterm_ind_list_Forall t);
-  [ intros xx; try (now intuition); simpl
-  | intros cc ll IHll; simpl;
-    rewrite ? flat_map_concat_map; rewrite ? map_map;
-    try f_equal;
+  apply (term_ind_list_Forall t);
+  [ intros nn; try (now intuition); simpl
+  | intros xx; try (now intuition); simpl
+  | intros cc ll IHll; simpl; intros;
+    try (apply (f_equal (tconstr _)));
+    rewrite ? flat_map_concat_map, ? map_map;
+    try (apply (f_equal (@concat _)));
+    match goal with
+    | |- map _ ?l = ?l => rewrite <- (map_id l) at 2
+    | _ => idtac
+    end;
     try (apply map_ext_in; intros i Hi; specialize_Forall_all i);
     try (apply Forall_forall; intros i Hi; specialize_Forall_all i);
     try (now intuition) ];
   try (now (rnow idtac)); try (now rcauto).
+
+Ltac formula_induction A :=
+  (try intros until A) ;
+  let XX := fresh "X" in
+  let xx := fresh "x" in
+  let ncon := fresh "ncon" in
+  let bcon := fresh "bcon" in
+  let qcon := fresh "qcon" in
+  let A1 := fresh A in
+  let A2 := fresh A in
+  let ll := fresh "l" in
+  let lll := fresh "l" in
+  let tt := fresh "t" in
+  let IHll := fresh "IHl" in
+  induction A as [ XX ll | ncon | bcon A1 ? A2 ? | qcon xx A ]; simpl; intros;
+  [ rewrite ? flat_map_concat_map;
+    try (apply (f_equal (fvar _)));
+    try (induction ll as [ | tt lll IHll ]; simpl; intuition;
+         rewrite IHll; f_equal; intuition)
+  | try ((try f_equal); intuition; fail)
+  | try (apply (f_equal2 (fbin _)));
+    intuition
+  | (try apply (f_equal (fqtf _ _))); repeat case_analysis; try (intuition; fail); 
+     try (intuition; (rnow idtac); fail) ];
+  try (now (rnow idtac)); try (now rcauto).
+
+
+Section H2N.
+
+Context { vatom : DecType } { tatom fatom : Type }.
+
+Arguments tvar {_} {_} {T} _.
+
+Notation hterm := (@term vatom tatom Empty_set).
+Notation hformula := (@formula vatom tatom fatom Nocon Icon Qcon Empty_set).
+
+Notation term := (@term vatom tatom nat).
+Notation formula := (@formula vatom tatom fatom Nocon Icon Qcon nat).
+Notation closed t := (tvars t = nil).
+Notation fclosed r := (forall n, closed (r n)).
+Notation "↑ r" := (felift r) (at level 25, format "↑ r").
+Notation "v // ↓ k" := (fesubs k v) (at level 18, format "v // ↓ k").
+Notation "A ⟦ r ⟧" := (esubs r A) (at level 8, left associativity, format "A ⟦ r ⟧").
+Notation "A [ u // x ]" := (subs x u A) (at level 8, format "A [ u // x ]").
+Notation "A [[ L ]]" := (multi_subs L A) (at level 8, format "A [[ L ]]").
+Notation "L ∖ x" := (remove_snd x L) (at level 18).
+Notation "⇑" := fup.
+Notation "A ↑" := (A⟦⇑⟧) (at level 8, format "A ↑").
+Notation "x ∈ A" := (In x (freevars A)) (at level 30).
+Notation "y #[ x ] A" := (no_capture_at x y A) (at level 30, format "y  #[ x ]  A").
+
+Infix "→" := (fbin imp_con) (at level 55, right associativity).
 
 Ltac run_ax :=
   match goal with
@@ -75,105 +88,106 @@ Ltac run_ax :=
   end.
 Ltac auto_ax := rewrite <- (app_nil_l _); run_ax.
 
-
-
-Fixpoint h2n_term (t : hterm) :=
+(* Translation of terms: trivial embedding *)
+Fixpoint h2n_term (t : hterm) : term :=
 match t with
-| hvar x => tvar x
-| hconstr f l => tconstr f (map h2n_term l)
+| tvar x => tvar x
+| dvar z => match z with end
+| tconstr f l => tconstr f (map h2n_term l)
 end.
 
-Lemma h2n_freevars : forall t, freevars (h2n_term t) = hfreevars t.
-Proof. hterm_induction t. Qed.
+Lemma h2n_tvars : forall t, tvars (h2n_term t) = tvars t.
+Proof. term_induction t. Qed.
 
-Lemma h2n_closed : forall t, hclosed t <-> closed (h2n_term t).
-Proof. intros t; rewrite h2n_freevars; intuition. Qed.
+Lemma h2n_closed : forall t, closed t <-> closed (h2n_term t).
+Proof. intros t; rewrite h2n_tvars; intuition. Qed.
 
 Lemma h2n_tsubs : forall x u t,
-  h2n_term (htsubs x u t) = tsubs x (h2n_term u) (h2n_term t).
-Proof. hterm_induction t. Qed.
+  h2n_term (tsubs x u t) = tsubs x (h2n_term u) (h2n_term t).
+Proof. term_induction t. Qed.
 Hint Rewrite h2n_tsubs : term_db.
 
-Lemma h2n_tup : forall k t, tup k (h2n_term t) = h2n_term t.
-Proof. hterm_induction t. Qed.
-Hint Rewrite h2n_tup : term_db.
+Lemma h2n_tesubs : forall r t, tesubs r (h2n_term t) = h2n_term t.
+Proof. term_induction t. Qed.
+Hint Rewrite h2n_tesubs : term_db.
 
-
-Fixpoint h2n_formula A : formula :=
+(* Translation of formulas: trivial embedding *)
+Fixpoint h2n_formula (A : hformula) : formula :=
 match A with
-| hfvar X l => var X (map h2n_term l)
-| himp B C => imp (h2n_formula B) (h2n_formula C)
-| hfrl y B => frl y (h2n_formula B)
-| hexs y B => exs y (h2n_formula B)
+| fvar X l => fvar X (map h2n_term l)
+| fnul _ ncon => match ncon with end
+| fbin bcon B C => fbin bcon (h2n_formula B) (h2n_formula C)
+| fqtf qcon y B => fqtf qcon y (h2n_formula B)
 end.
 
-Lemma h2n_ffreevars : forall A, ffreevars (h2n_formula A) = hffreevars A.
-Proof. formula_induction A; apply h2n_freevars. Qed.
+Lemma h2n_freevars : forall A, freevars (h2n_formula A) = freevars A.
+Proof. formula_induction A; (try now rewrite ? IHA1, ? IHA2, ? IHA); apply h2n_tvars. Qed.
 
-Lemma h2n_fclosed : forall A, hffreevars A = nil <-> ffreevars (h2n_formula A) = nil.
-Proof. intros A; rewrite h2n_ffreevars; intuition. Qed.
+Lemma h2n_closed_formula : forall A, freevars A = nil <-> freevars (h2n_formula A) = nil.
+Proof. intros A; rewrite h2n_freevars; intuition. Qed.
 
-Lemma h2n_fsubs : forall x u A,
-  h2n_formula (hfsubs x u A) = subs x (h2n_term u) (h2n_formula A).
+Lemma h2n_subs : forall x u A,
+  h2n_formula (A[u//x]) = (h2n_formula A)[h2n_term u//x].
 Proof. formula_induction A. Qed.
-Hint Rewrite h2n_fsubs : term_db.
+Hint Rewrite h2n_subs : term_db.
 
-Lemma h2n_fup : forall k A, fup k (h2n_formula A) = h2n_formula A.
+Lemma h2n_esubs : forall r A, (h2n_formula A)⟦r⟧ = h2n_formula A.
 Proof. formula_induction A. Qed.
-Hint Rewrite h2n_fup : term_db.
+Hint Rewrite h2n_esubs : term_db.
 
-Lemma h2n_good_for : forall x y A, hgood_for x y A -> good_for x y (h2n_formula A).
-Proof. formula_induction A; rewrite h2n_ffreevars in H0; intuition. Qed.
+Lemma h2n_no_capture : forall x y A, y #[x] A -> y #[x] (h2n_formula A).
+Proof. formula_induction A; rewrite h2n_freevars in H0; intuition. Qed.
 
 Proposition h2n : forall A, hprove A ->
-  forall L, Forall (fun z => closed z) (map snd L) -> incl (hffreevars A) (map fst L) ->
-  prove nil (multi_subs L (h2n_formula A)).
+  forall L, Forall (fun z => closed z) (map snd L) -> incl (freevars A) (map fst L) ->
+  prove nil (h2n_formula A)[[L]].
 Proof.
 intros A pi; induction pi; intros L Hcl Hsub;
-  simpl; rewrite ? multi_subs_imp;
-  remember (multi_subs L (h2n_formula A)) as AA;
-  (try remember (multi_subs L (h2n_formula B)) as BB);
-  (try remember (multi_subs L (h2n_formula C)) as CC);
+  simpl; rewrite ? multi_subs_fbin;
+  remember ((h2n_formula A)[[L]]) as AA;
+  (try remember ((h2n_formula B)[[L]]) as BB);
+  (try remember ((h2n_formula C)[[L]]) as CC);
   repeat apply impi.
 - change (BB :: AA :: nil) with ((BB :: nil) ++ AA :: nil); apply ax.
 - apply (impe BB).
   + apply (impe AA).
-    * change (AA :: imp AA BB :: imp AA (imp BB CC) :: nil)
-        with ((AA :: imp AA BB :: nil) ++ imp AA (imp BB CC) :: nil); apply ax.
+    * change (AA :: AA → BB :: AA → BB → CC :: nil)
+        with ((AA :: AA → BB :: nil) ++ AA → BB → CC :: nil); apply ax.
     * apply ax_hd.
   + apply (impe AA).
-    * change (AA :: imp AA BB :: imp AA (imp BB CC) :: nil)
-        with ((AA :: nil) ++ imp AA BB :: imp AA (imp BB CC) :: nil); apply ax.
+    * change (AA :: AA → BB :: AA → BB → CC :: nil)
+        with ((AA :: nil) ++ AA → BB :: AA → BB → CC :: nil); apply ax.
     * apply ax_hd.
-- remember (map (fun x => (x, dvar 0 : term)) (hffreevars A)) as LA.
+- remember (map (fun x => (x, dvar 0 : term)) (freevars A)) as LA.
   assert (Forall (fun z => closed z) (map snd LA)) as HcLA
-    by (subst LA; remember (hffreevars A) as l; clear; induction l; simpl; intuition).
-  assert (map fst LA = hffreevars A) as HfstLA
-    by (subst LA; remember (hffreevars A) as l; clear; induction l; simpl; try rewrite IHl; intuition).
-  remember (multi_subs (L ++ LA) (h2n_formula A)) as AAA.
+    by (subst LA; remember (freevars A) as l; clear; induction l; simpl; intuition).
+  assert (map fst LA = freevars A) as HfstLA
+    by (subst LA; remember (freevars A) as l; clear;
+          induction l; simpl; try rewrite IHl; intuition).
+  remember ((h2n_formula A)[[L ++ LA]]) as AAA.
   apply (impe AAA).
   + specialize IHpi1 with (L ++ LA).
-    simpl in IHpi1; rewrite ? multi_subs_imp in IHpi1.
-    subst AAA BB; rewrite multi_subs_ext with L (h2n_formula B) LA;
-      [ apply IHpi1 | assumption | rewrite h2n_ffreevars ]; rewrite ? map_app; intuition.
+    simpl in IHpi1; rewrite ? multi_subs_fbin in IHpi1.
+    subst AAA BB; rewrite multi_subs_ext with (L':= LA) (A0:= h2n_formula B);
+      [ apply IHpi1 | assumption | rewrite h2n_freevars ]; rewrite ? map_app; intuition.
     * apply Forall_app; intuition.
     * apply incl_app; [ apply incl_appr | apply incl_appl ]; intuition.
       rewrite HfstLA; apply incl_refl.
   + subst AAA; apply IHpi2; rewrite ? map_app.
     * apply Forall_app; intuition.
     * apply incl_appr; rewrite HfstLA; apply incl_refl.
-- rewrite multi_subs_frl, h2n_fsubs, multi_subs_subs; intuition.
-  + destruct (in_dec eq_dt_dec x (ffreevars (h2n_formula A))) as [Hf|Hf].
+- rewrite multi_subs_fqtf, h2n_subs, multi_subs_subs; intuition.
+  + destruct (in_dec eq_dt_dec x (freevars (h2n_formula A))) as [Hf|Hf].
     * apply frle; [ | apply ax_hd ].
       clear - f Hcl Hsub Hf.
-      apply multi_tsubs_is_closed; [ assumption | ].
+      apply multi_tsubs_closed; [ assumption | ].
       intros z Hinz.
       apply Hsub; simpl.
-      rewrite h2n_ffreevars in Hf; rewrite h2n_freevars in Hinz.
-      apply hffreevars_to_subs with (x0:= z) (t0:= t) in Hf; intuition.
+      rewrite h2n_freevars in Hf; rewrite h2n_tvars in Hinz.
+      apply no_capture_subs_freevars with (x0:= z) (u:= t) in Hf; intuition.
       now specialize_Forall f with z.
-    * assert (~ In x (ffreevars (multi_subs (remove_snd x L) (h2n_formula A)))) as Hnin.
-      { intros Hin; apply Hf; apply multi_subs_ffreevars in Hin; try assumption.
+    * assert (~ x ∈ (h2n_formula A)[[L ∖ x]]) as Hnin.
+      { intros Hin; apply Hf; apply multi_subs_freevars in Hin; try assumption.
         apply Forall_incl with (map snd L); intuition.
         clear; induction L; intuition; simpl; case_analysis; intuition. }
       rewrite nfree_subs by assumption.
@@ -182,35 +196,31 @@ intros A pi; induction pi; intros L Hcl Hsub;
       rewrite nfree_subs by assumption.
       apply ax_hd.
   + apply Forall_forall; intros z Hinz.
-    rewrite h2n_freevars in Hinz.
+    rewrite h2n_tvars in Hinz.
     specialize_Forall f with z.
-    now apply h2n_good_for.
-- rewrite ? multi_subs_frl.
+    now apply h2n_no_capture.
+- rewrite ? multi_subs_fqtf.
   rewrite <- @multi_subs_remove with (x:=x) in HeqAA; try assumption.
   + apply frli; simpl.
-    apply impe with (fup 0 AA); [ | apply ax_hd ].
-    rewrite multi_subs_imp; simpl; rewrite <- HeqAA.
-    replace (imp (fup 0 AA) (subs x (dvar 0)
-                                (fup 0 (multi_subs (remove_snd x L) (h2n_formula B)))))
-       with (subs x (dvar 0) (imp (fup 0 AA)
-                                (fup 0 (multi_subs (remove_snd x L) (h2n_formula B))))).
+    apply impe with (AA↑); [ | apply ax_hd ].
+    rewrite multi_subs_fbin; simpl; rewrite <- HeqAA.
+    replace (AA↑ → (h2n_formula B)[[L ∖ x]]↑[dvar 0//x])
+       with ((AA↑ → (h2n_formula B)[[L ∖ x]]↑)[dvar 0//x]).
     { apply frle; intuition; auto_ax. }
     simpl; f_equal; apply nfree_subs.
     intros Hin; apply n.
-    rewrite ffreevars_fup in Hin; subst.
-    apply multi_subs_ffreevars in Hin.
-    * now rewrite <- h2n_ffreevars.
+    rewrite freevars_fup in Hin; subst.
+    apply multi_subs_freevars in Hin.
+    * now rewrite <- h2n_freevars.
     * apply Forall_incl with (map snd L); intuition.
       clear; induction L; intuition; simpl; case_analysis; intuition.
-  + now rewrite h2n_ffreevars.
-- rewrite multi_subs_frl.
+  + now rewrite h2n_freevars.
+- rewrite multi_subs_fqtf.
   apply frli; simpl.
-  rewrite fup_multi_subs, h2n_fup.
-  replace (subs x (dvar 0)
-          (multi_subs (map (fun x0 => (fst x0, tup 0 (snd x0))) (remove_snd x L))
-             (h2n_formula A)))
-     with (multi_subs ((map (fun x0 => (fst x0, tup 0 (snd x0))) (remove_snd x L) ++
-             (x, dvar 0) :: nil)) (h2n_formula A))
+  rewrite multi_subs_esubs, h2n_esubs by (apply Forall_forall; intuition).
+  replace (((h2n_formula A)[[map (fun '(x0, u) => (x0, tesubs ⇑ u)) (L ∖ x)]])[dvar 0//x])
+     with (((h2n_formula A)[[map (fun '(x0, u) => (x0, tesubs ⇑ u)) (L ∖ x)
+                             ++ (x, dvar 0) :: nil]]))
     by now unfold multi_subs; rewrite fold_left_app; simpl.
   apply IHpi.
   + rewrite map_app; apply Forall_app.
@@ -218,25 +228,28 @@ intros A pi; induction pi; intros L Hcl Hsub;
       revert Hcl; clear; induction L; simpl; intros HF; [ now constructor | destruct a ].
       simpl in HF; inversion_clear HF.
       case_analysis; intuition; constructor; rcauto.
+      now rewrite tvars_fup.
     * now repeat constructor.
   + clear - Hsub; simpl in Hsub.
     intros z Hinz.
-    revert Hsub; case (eq_dt_reflect z x); intros Heq Hsub; subst; rewrite map_app; simpl; try in_solve.
-    rewrite map_map; simpl; rewrite <- remove_snd_remove.
+    revert Hsub; case (eq_dt_reflect z x); intros Heq Hsub; subst;
+      rewrite map_app; simpl; try in_solve.
+    rewrite map_map, map_ext with (g:= fst) by (intros [? ?]; reflexivity).
+    rewrite <- remove_snd_remove.
     eapply notin_remove with (y:= x) in Hinz; intuition ; apply Hsub in Hinz.
     apply notin_remove with (Hdec:= eq_dt_dec) (y:= x) in Hinz; intuition.
-- rewrite multi_subs_exs, h2n_fsubs, multi_subs_subs; try assumption.
-  + destruct (in_dec eq_dt_dec x (ffreevars (h2n_formula A))) as [Hf|Hf].
+- rewrite multi_subs_fqtf, h2n_subs, multi_subs_subs; try assumption.
+  + destruct (in_dec eq_dt_dec x (freevars (h2n_formula A))) as [Hf|Hf].
     * eapply exsi; [ | apply ax_hd ].
       clear - f Hcl Hsub Hf.
-      apply multi_tsubs_is_closed; [ assumption | ].
+      apply multi_tsubs_closed; [ assumption | ].
       intros z Hinz.
       apply Hsub; simpl.
-      rewrite h2n_ffreevars in Hf; rewrite h2n_freevars in Hinz.
-      apply hffreevars_to_subs with (x0:= z) (t0:= t) in Hf; intuition.
+      rewrite h2n_freevars in Hf; rewrite h2n_tvars in Hinz.
+      apply no_capture_subs_freevars with (x0:= z) (u:= t) in Hf; intuition.
       now specialize_Forall f with z.
-    * assert (~ In x (ffreevars (multi_subs (remove_snd x L) (h2n_formula A)))) as Hnin.
-      { intros Hin; apply Hf; apply multi_subs_ffreevars in Hin; try assumption.
+    * assert (~ x ∈ (h2n_formula A)[[L ∖ x]]) as Hnin.
+      { intros Hin; apply Hf; apply multi_subs_freevars in Hin; try assumption.
         apply Forall_incl with (map snd L); intuition.
         clear; induction L; intuition; simpl; case_analysis; intuition. }
       rewrite nfree_subs by assumption.
@@ -244,25 +257,24 @@ intros A pi; induction pi; intros L Hcl Hsub;
       rewrite nfree_subs by assumption.
       apply ax_hd.
   + apply Forall_forall; intros z Hinz.
-    rewrite h2n_freevars in Hinz.
+    rewrite h2n_tvars in Hinz.
     specialize_Forall f with z.
-    now apply h2n_good_for.
-- rewrite multi_subs_frl, multi_subs_exs.
+    now apply h2n_no_capture.
+- rewrite 2 multi_subs_fqtf.
   rewrite <- @multi_subs_remove with (x:=x) in HeqBB; try assumption.
-  + apply @exse with (x:=x) (A:=multi_subs (remove_snd x L) (h2n_formula A)); [ apply ax_hd | ].
-    apply impe with (subs x (dvar 0) (fup 0 (multi_subs (remove_snd x L) (h2n_formula A))));
-      [ | apply ax_hd ].
-    replace (imp (subs x (dvar 0) (fup 0 (multi_subs (remove_snd x L) (h2n_formula A)))) (fup 0 BB))
-       with (subs x (dvar 0) (imp (fup 0 (multi_subs (remove_snd x L) (h2n_formula A))) (fup 0 BB))).
-    { apply frle; [ reflexivity | simpl; rewrite multi_subs_imp; subst; auto_ax ]. }
+  + apply @exse with (x:=x) (A:= (h2n_formula A)[[L ∖ x]]); [ apply ax_hd | ].
+    apply impe with ((h2n_formula A)[[L ∖ x]]↑[dvar 0//x]); [ | apply ax_hd ].
+    replace ((h2n_formula A)[[L ∖ x]]↑[dvar 0//x] → BB↑)
+       with (((h2n_formula A)[[L ∖ x]]↑ → BB↑)[dvar 0//x]).
+    { apply frle; [ reflexivity | simpl; rewrite multi_subs_fbin; subst; auto_ax ]. }
     simpl; f_equal; apply nfree_subs.
     intros Hin; apply n.
-    rewrite ffreevars_fup in Hin; subst.
-    apply multi_subs_ffreevars in Hin.
-    * now rewrite <- h2n_ffreevars.
+    rewrite freevars_fup in Hin; subst.
+    apply multi_subs_freevars in Hin.
+    * now rewrite <- h2n_freevars.
     * apply Forall_incl with (map snd L); intuition.
       clear; induction L; intuition; simpl; case_analysis; intuition.
-  + now rewrite h2n_ffreevars.
+  + now rewrite h2n_freevars.
 Qed.
 
 End H2N.
