nj2hilbert.v
@@ -4,54 +4,6 @@ Require Import stdlib_more.
 Require Export nj1 hilbert.
 
 
-Section N2H.
-
-Context { vatom : InfDecType } { tatom : Type } { fatom : Type }.
-Notation vfresh := (@fresh vatom).
-Notation vfresh_prop := (@fresh_prop vatom).
-Notation term := (@term vatom tatom).
-Notation closed t := (freevars t = nil).
-Notation tup := (@tup vatom tatom).
-Notation hterm := (@hterm vatom tatom).
-Notation hclosed t := (hfreevars t = nil).
-Notation formula := (@formula vatom tatom fatom).
-Notation hformula := (@hformula vatom tatom fatom).
-Infix "⟶" := himp (at level 70, right associativity).
-
-Hint Rewrite
-  (@tup_tup_com vatom tatom) (@tup_tsubs_com vatom tatom)
-  (@ntsubs_tup_com vatom tatom) (@ntsubs_z_tup vatom tatom)
-  (@freevars_tup vatom tatom) (@tsubs_tsubs_eq vatom tatom) : term_db.
-Hint Resolve (@closed_nofreevars vatom tatom) : term_db.
-Hint Rewrite (@freevars_ntsubs vatom tatom) using intuition; fail : term_db.
-Hint Rewrite (@nfree_tsubs vatom tatom)
-  using try (intuition; fail); (try apply closed_nofreevars); intuition; fail : term_db.
-Hint Rewrite (@ntsubs_tsubs_com vatom tatom)
-  using try (intuition; fail); (try apply closed_nofreevars); intuition; fail : term_db.
-Hint Rewrite (@tsubs_tsubs_com vatom tatom)
-  using try (intuition; fail); (try apply closed_nofreevars); intuition; fail : term_db.
-Hint Rewrite (@freevars_tsubs_closed vatom tatom)
-  using intuition; fail : term_db.
-
-Ltac formula_induction A :=
-  (try intros until A) ;
-  let XX := fresh "X" in
-  let xx := fresh "x" in
-  let A1 := fresh A in
-  let A2 := fresh A in
-  let ll := fresh "l" in
-  let lll := fresh "l" in
-  let tt := fresh "t" in
-  let IHll := fresh "IHl" in
-  induction A as [ XX ll | A1 ? A2 ? | xx A | xx A ]; simpl; intros;
-  [ rewrite ? flat_map_concat_map;
-    try f_equal; try (induction ll as [ | tt lll IHll ]; simpl; intuition;
-                      rewrite IHll; f_equal; intuition)
-  | try (f_equal; intuition)
-  | try (repeat case_analysis; intuition; f_equal; intuition; (rnow idtac); fail)
-  | try (repeat case_analysis; intuition; f_equal; intuition; (rnow idtac); fail) ];
-  try (now (rnow idtac)); try (now rcauto).
-
 Ltac term_induction t :=
   (try intros until t);
   let nn := fresh "n" in
@@ -64,258 +16,102 @@ Ltac term_induction t :=
   apply (term_ind_list_Forall t);
   [ intros nn; try (now intuition); simpl
   | intros xx; try (now intuition); simpl
-  | intros cc ll IHll; simpl;
-    rewrite ? flat_map_concat_map; rewrite ? map_map;
-    try f_equal;
+  | intros cc ll IHll; simpl; intros;
+    try (apply (f_equal (tconstr _)));
+    rewrite ? flat_map_concat_map, ? map_map;
+    try (apply (f_equal (@concat _)));
+    match goal with
+    | |- map _ ?l = ?l => rewrite <- (map_id l) at 2
+    | _ => idtac
+    end;
     try (apply map_ext_in; intros i Hi; specialize_Forall_all i);
     try (apply Forall_forall; intros i Hi; specialize_Forall_all i);
     try (now intuition) ];
   try (now (rnow idtac)); try (now rcauto).
 
-Ltac hterm_induction t :=
-  (try intros until t);
-  let nn := fresh "n" in
+Ltac formula_induction A :=
+  (try intros until A) ;
+  let XX := fresh "X" in
   let xx := fresh "x" in
-  let cc := fresh "c" in
+  let ncon := fresh "ncon" in
+  let bcon := fresh "bcon" in
+  let qcon := fresh "qcon" in
+  let A1 := fresh A in
+  let A2 := fresh A in
   let ll := fresh "l" in
+  let lll := fresh "l" in
+  let tt := fresh "t" in
   let IHll := fresh "IHl" in
-  let i := fresh "i" in
-  let Hi := fresh "Hi" in
-  apply (hterm_ind_list_Forall t);
-  [ intros xx; try (now intuition); simpl
-  | intros cc ll IHll; simpl;
-    rewrite ? flat_map_concat_map; rewrite ? map_map;
-    try f_equal;
-    try (apply map_ext_in; intros i Hi; specialize_Forall_all i);
-    try (apply Forall_forall; intros i Hi; specialize_Forall_all i);
-    try (now intuition) ];
+  induction A as [ XX ll | ncon | bcon A1 ? A2 ? | qcon xx A ]; simpl; intros;
+  [ rewrite ? flat_map_concat_map;
+    try (apply (f_equal (fvar _)));
+    try (induction ll as [ | tt lll IHll ]; simpl; intuition;
+         rewrite IHll; f_equal; intuition)
+  | try ((try f_equal); intuition; fail)
+  | try (apply (f_equal2 (fbin _)));
+    intuition
+  | (try apply (f_equal (fqtf _ _))); repeat case_analysis; try (intuition; fail); 
+     try (intuition; (rnow idtac); fail) ];
   try (now (rnow idtac)); try (now rcauto).
+
+
+Section N2H.
+
+Context { vatom : InfDecType } { tatom fatom : Type }.
+
+Arguments tvar {_} {_} {T} _.
+
+Notation hterm := (@term vatom tatom Empty_set).
+Notation hformula := (@formula vatom tatom fatom Nocon Icon Qcon Empty_set).
+
+Notation term := (@term vatom tatom nat).
+Notation formula := (@formula vatom tatom fatom Nocon Icon Qcon nat).
+Notation closed t := (tvars t = nil).
+Notation fclosed r := (forall n, closed (r n)).
+Notation "↑ r" := (felift r) (at level 25, format "↑ r").
+Notation "v // ↓ k" := (fesubs k v) (at level 18, format "v // ↓ k").
+Notation "A ⟦ r ⟧" := (esubs r A) (at level 8, left associativity, format "A ⟦ r ⟧").
+Notation "A [ u // x ]" := (subs x u A) (at level 8, format "A [ u // x ]").
+Notation "A [[ L ]]" := (multi_subs L A) (at level 8, format "A [[ L ]]").
+Notation "L ∖ x" := (remove_snd x L) (at level 18).
+Notation "⇑" := fup.
+Notation "A ↑" := (A⟦⇑⟧) (at level 8, format "A ↑").
+Notation "x ∈ A" := (In x (freevars A)) (at level 30).
+Notation "y #[ x ] A" := (no_capture_at x y A) (at level 30, format "y  #[ x ]  A").
+Notation "r #[[ l ]] A" := (no_ecapture_at r l A) (at level 30, format "r  #[[ l ]]  A").
+
+Infix "→" := (fbin imp_con) (at level 55, right associativity).
+
+(*
+Hint Rewrite
+  (@tup_tup_com vatom tatom) (@tup_tsubs_com vatom tatom)
+  (@ntsubs_tup_com vatom tatom) (@ntsubs_z_tup vatom tatom)
+  (@freevars_tup vatom tatom) (@tsubs_tsubs_eq vatom tatom) : term_e.
+Hint Resolve (@closed_nofreevars vatom tatom) : term_e.
+Hint Rewrite (@freevars_ntsubs vatom tatom) using intuition; fail : term_e.
+Hint Rewrite (@nfree_tsubs vatom tatom)
+  using try (intuition; fail); (try apply closed_nofreevars); intuition; fail : term_e.
+Hint Rewrite (@ntsubs_tsubs_com vatom tatom)
+  using try (intuition; fail); (try apply closed_nofreevars); intuition; fail : term_e.
+Hint Rewrite (@tsubs_tsubs_com vatom tatom)
+  using try (intuition; fail); (try apply closed_nofreevars); intuition; fail : term_e.
+Hint Rewrite (@freevars_tsubs_closed vatom tatom)
+  using intuition; fail : term_e.
+*)
 
 
 Section Fixed_r.
 
 Variable r : nat -> hterm.
 
-(* Capture-avoiding property *)
-Fixpoint ltgood_for lv (t : term) :=
-match t with
-| dvar n => Forall (fun x => ~ In x (hfreevars (r n))) lv
-| tvar x => True
-| tconstr f l => fold_right (fun x P => and (ltgood_for lv x) P) True l
-end.
-
-Lemma ltgood_for_less : forall x lv1 lv2 t,
-  ltgood_for (lv1 ++ x :: lv2) t -> ltgood_for (lv1 ++ lv2) t.
-Proof. term_induction t; intros HF.
-- apply Forall_incl with (lv1 ++ x :: lv2); intuition.
-- apply Forall_fold_right in HF.
-  apply Forall_fold_right, Forall_forall; intros u Hu.
-  specialize_Forall_all u; intuition.
-Qed.
-
-Lemma ltgood_for_closed : forall l t, (forall n, hclosed (r n)) -> ltgood_for l t.
-Proof. intros l t Hc; term_induction t.
-- rewrite (Hc n).
-  apply Forall_forall; auto.
-- now apply Forall_fold_right.
-Qed.
-
-Fixpoint lgood_for lv (A : formula) :=
-match A with
-| var X l => fold_right (fun x P => and (ltgood_for lv x) P) True l
-| imp B C => lgood_for lv B /\ lgood_for lv C
-| frl z B => lgood_for (z :: lv) B
-| exs z B => lgood_for (z :: lv) B
-end.
-
-Lemma lgood_for_less : forall x lv1 lv2 A,
-  lgood_for (lv1 ++ x :: lv2) A -> lgood_for (lv1 ++ lv2) A.
-Proof. intros x lv1 lv2 A; revert lv1 lv2; formula_induction A.
-- apply Forall_fold_right in H; apply Forall_fold_right.
-  eapply Forall_impl; [ apply ltgood_for_less | eassumption ].
-- now rewrite app_comm_cons in H; apply IHA in H.
-- now rewrite app_comm_cons in H; apply IHA in H.
-Qed.
-
-Lemma lgood_for_closed : forall l A, (forall n, hclosed (r n)) -> lgood_for l A.
-Proof. intros l A Hc; revert l; formula_induction A.
-apply Forall_fold_right.
-apply Forall_forall; intros.
-now apply ltgood_for_closed.
-Qed.
-
-
-Fixpoint n2h_term t :=
-match t with
-| dvar n => r n
-| tvar x => hvar x
-| tconstr f l => hconstr f (map n2h_term l)
-end.
-
-Lemma n2h_hfreevars : forall t, incl (freevars t) (hfreevars (n2h_term t)).
-Proof. term_induction t; intros z Hin.
-revert IHl Hin; induction l; simpl; intros Hl Hin; auto.
-inversion Hl; subst; in_solve.
-Qed.
-
-Fixpoint n2h_formula (A : formula) :=
-match A with
-| var X l => hfvar X (map n2h_term l)
-| imp B C => himp (n2h_formula B) (n2h_formula C)
-| frl y B => hfrl y (n2h_formula B)
-| exs y B => hexs y (n2h_formula B)
-end.
-
-Lemma n2h_tsubs : forall x u t lv, In x lv -> ltgood_for lv t ->
-  n2h_term (tsubs x u t) = htsubs x (n2h_term u) (n2h_term t).
-Proof. term_induction t; intros lv Hin Hg.
-- specialize_Forall Hg with x.
-  symmetry; now apply nfree_htsubs.
-- apply Forall_fold_right in Hg.
-  f_equal; apply map_ext_in; intros a Hina.
-  now specialize_Forall_all a; apply (IHl _ Hin).
-Qed.
-
-Lemma n2h_subs : forall x u A lv, In x lv -> lgood_for lv A ->
-  n2h_formula (subs x u A) = hfsubs x (n2h_term u) (n2h_formula A).
-Proof. formula_induction A.
-- now simpl in H0; apply n2h_tsubs with lv.
-- now simpl in H0.
-- now apply IHA1 with lv.
-- now apply IHA2 with lv.
-- case_analysis; [ reflexivity | ].
-  rewrite <- (app_nil_l _) in H0; apply lgood_for_less in H0.
-  now f_equal; apply IHA with lv.
-- case_analysis; [ reflexivity | ].
-  rewrite <- (app_nil_l _) in H0; apply lgood_for_less in H0.
-  now f_equal; apply IHA with lv.
-Qed.
-
-Lemma n2h_allvars : forall A,
-  incl (allvars A ++ hffreevars (n2h_formula A)) (hallvars (n2h_formula A)).
-Proof. formula_induction A; simpl; intros z Hin; try in_solve.
-- revert Hin; induction l; simpl; intros Hin; try in_solve.
-  apply in_app_or in Hin; destruct Hin as [Hin|Hin]; auto.
-  apply in_or_app; apply in_app_or in Hin; destruct Hin as [Hin|Hin]; [left|right]; intuition.
-  now apply n2h_hfreevars.
-- refine ?[mygoal]. Existential 1 := ?mygoal.
-  inversion_clear Hin; subst; intuition.
-  apply in_cons, IHA.
-  apply in_or_app; apply in_app_or in H; destruct H as [H|H]; [left|right]; auto.
-  now apply in_remove in H.
-Qed.
-
-
-(* Properties relating [lgood_for] and [n2h] *)
-Lemma ltgood_for_nfree : forall y l u,
-  closed u -> In y l -> ltgood_for l u -> ~ In y (hfreevars (n2h_term u)).
-Proof. intros y l u; revert l; term_induction u; intros lv Hc Hinl Hg Hinu.
-- specialize_Forall Hg with y; intuition.
-- apply concat_is_nil in Hc.
-  apply Forall_fold_right in Hg.
-  apply in_flat_map in Hinu; destruct Hinu as [z [Hinzl Hinz]].
-  apply in_map_iff in Hinzl.
-  destruct Hinzl as [v [Heq Hz]]; subst.
-  specialize_Forall_all v.
-  apply in_map with (f:= freevars) in Hz.
-  specialize_Forall Hc with (freevars v).
-  apply IHl in Hg; intuition.
-Qed.
-
-Lemma ltgood_for_freevars : forall x l t, In x l -> ltgood_for l t ->
-  In x (hfreevars (n2h_term t)) -> In x (freevars t).
-Proof. intros x l t; revert l; term_induction t; intros lv Hinlv Hg Hin.
-- now specialize_Forall Hg with x.
-- apply Forall_fold_right in Hg.
-  apply in_flat_map_Exists in Hin; apply Exists_exists in Hin.
-  destruct Hin as [lv2 [Hlv2in Hinlv2]].
-  apply in_map_iff in Hlv2in; destruct Hlv2in as [u [Heq Hinu]]; subst.
-  specialize_Forall_all u.
-  apply IHl with lv in Hinlv2; intuition.
-  rewrite <- flat_map_concat_map; apply in_flat_map; exists u; intuition.
-Qed.
-
-Lemma ltgood_for_nfree_subs : forall x y l u t,
-  closed u -> In y l -> ltgood_for l (tsubs x u t) ->
-  In y (hfreevars (n2h_term u)) -> In x (freevars t) -> False.
-Proof. intros x y l u t; revert l; term_induction t; intros lv Hc Hinl Hg Hinu Hint.
-- destruct Hint; subst; intuition.
-  revert Hg; case_analysis; intros Hg.
-  now apply ltgood_for_nfree with (y:= y) in Hg.
-- apply Forall_fold_right in Hg.
-  apply in_flat_map in Hint; destruct Hint as [z [Hinzl Hinz]].
-  apply in_map_iff in Hinzl.
-  destruct Hinzl as [v [Heq Hz]]; subst.
-  specialize_Forall_all v.
-  apply in_map with (f:= tsubs x u) in Hz.
-  specialize_Forall Hg with (tsubs x u v).
-  apply IHl in Hg; intuition.
-Qed.
-
-Lemma lgood_for_nfree_subs : forall x y l u A,
-  closed u -> In y l -> lgood_for l (subs x u A) ->
-  In y (hfreevars (n2h_term u)) -> In x (ffreevars A) -> False.
-Proof. intros x y l u A; revert l; formula_induction A.
-- apply Forall_fold_right in H1.
-  apply in_flat_map in H3; destruct H3 as [z [Hinzl Hinz]].
-  apply in_map with (f:= tsubs x u) in Hinzl.
-  specialize_Forall H1 with (tsubs x u z).
-  apply ltgood_for_nfree_subs with (y:= y) in H1; intuition.
-- apply in_app_or in H3; destruct H3.
-  + now apply IHA1 with l.
-  + now apply IHA2 with l.
-- refine ?[mygoal]. Existential 1 := ?mygoal.
-  apply in_remove in H3; destruct H3 as [Hin Hneq].
-  revert H1; case_analysis; intros Hg; intuition.
-  rewrite <- (app_nil_l _) in Hg; apply lgood_for_less in Hg; simpl in Hg.
-  apply IHA in Hg; intuition.
-Qed.
-
-Lemma lgood_for_ffreevars : forall x l A, In x l -> lgood_for l A ->
-  In x (hffreevars (n2h_formula A)) -> In x (ffreevars A).
-Proof. intros x l A; revert l; formula_induction A.
-- apply in_flat_map in H1; destruct H1 as [t [Htin Hint]].
-  apply in_map_iff in Htin; destruct Htin as [y [Heq Hiny]]; subst.
-  apply Forall_fold_right in H0; specialize_Forall H0 with y.
-  apply ltgood_for_freevars with (l:= l0) in Hint; intuition.
-  rewrite <- flat_map_concat_map; apply in_flat_map; exists y; intuition.
-- apply in_or_app; apply in_app_or in H1; destruct H1; [left|right].
-  + now apply IHA1 with l.
-  + now apply IHA2 with l.
-- refine ?[mygoal]. Existential 1 := ?mygoal.
-  apply in_remove in H1; destruct H1 as [Hin Hneq].
-  apply notin_remove; intuition.
-  apply IHA with (x0 :: l); intuition.
-Qed.
-
-Lemma lgood_hgood_closed : forall u x lv lv' A,
-  closed u -> lgood_for lv (subs x u A) -> In x lv' -> lgood_for lv' A ->
-  Forall (fun y => hgood_for x y (n2h_formula A)) (hfreevars (n2h_term u)).
-Proof. intros u x lv lv' A; revert lv; formula_induction A.
-- now apply Forall_forall.
-- apply Forall_and.
-  + now apply IHA1 with lv.
-  + now apply IHA2 with lv.
-- refine ?[mygoal]. Existential 1 := ?mygoal.
-  revert H0; case_analysis; intros H0.
-  + apply Forall_forall; intros z Hz Hin.
-    exfalso; now apply in_remove in Hin.
-  + rewrite <- (app_nil_l _) in H2; apply lgood_for_less in H2; simpl in H2.
-    assert (Hg := H0).
-    apply IHA in H0; auto.
-    apply Forall_forall; intros z Hz Hin.
-    specialize_Forall H0 with z; split; [ assumption | ].
-    intros Heq2; subst.
-    apply in_remove in Hin; destruct Hin as [Hin _].
-    apply lgood_for_ffreevars with (l:= lv') in Hin; intuition.
-    apply lgood_for_nfree_subs with (y:= x0) in Hg; intuition.
-Qed.
-
+Notation n2h_term := (tesubs r).
+Notation n2h_formula := (esubs r).
 
 (* Turn sequents into formulas *)
-Definition s2f l (A : formula) := fold_left (fun x y => imp y x) l A.
+Definition s2f l (A : formula) := fold_left (fun x y => y → x) l A.
 
-Lemma good_for_s2f : forall lv l A, lgood_for lv (s2f l A) <-> Forall (lgood_for lv) (A :: l).
+Lemma no_ecapture_s2f : forall lv l A,
+  r #[[lv]] (s2f l A) <-> Forall (no_ecapture_at r lv) (A :: l).
 Proof.
 induction l; simpl; intros A; split; intros Hg; intuition.
 - inversion_clear Hg; intuition.
@@ -325,13 +121,13 @@ Qed.
 
 Notation n2h_sequent l A := (n2h_formula (s2f l A)).
 
-Lemma n2h_sequent_allvars : forall l A,
-  incl (hallvars (n2h_sequent l A))
-       (hallvars (n2h_formula A) ++ flat_map (fun C => hallvars (n2h_formula C)) l).
+Lemma n2h_sequent_fvars : forall l A,
+  incl (fvars (n2h_sequent l A))
+       (fvars (n2h_formula A) ++ flat_map (fun C => fvars (n2h_formula C)) l).
 Proof. induction l; simpl; intros A C HC; intuition; apply IHl in HC; in_solve. Qed.
 
 Lemma hprove_Bsequent : forall l A B,
-  hprove ((n2h_formula A ⟶ n2h_formula B) ⟶ n2h_sequent l A ⟶ n2h_sequent l B).
+  hprove ((n2h_formula A → n2h_formula B) → n2h_sequent l A → n2h_sequent l B).
 Proof.
 induction l; simpl; intros A B.
 - apply hprove_I.
@@ -356,7 +152,7 @@ eapply hprove_MP; [ eapply hprove_MP; [ apply hprove_Bsequent | apply hprove_K ]
 Qed.
 
 Lemma hprove_Ssequent : forall l A B,
-  hprove (n2h_sequent l (imp A B) ⟶ n2h_sequent l A ⟶ n2h_sequent l B).
+  hprove (n2h_sequent l (imp A B) → n2h_sequent l A → n2h_sequent l B).
 Proof.
 induction l; simpl; intros A B.
 - apply hprove_I.
@@ -366,7 +162,7 @@ induction l; simpl; intros A B.
 Qed.
 
 Lemma hprove_sequent_imp : forall l A B,
-  hprove (n2h_sequent l (imp A B)) -> hprove (n2h_formula A ⟶ n2h_sequent l B).
+  hprove (n2h_sequent l (imp A B)) -> hprove (n2h_formula A → n2h_sequent l B).
 Proof.
 induction l; simpl; intros A B pi; auto.
 apply IHl.
@@ -375,7 +171,7 @@ apply hprove_C.
 Qed.
 
 Lemma hprove_imp_sequent : forall l A B,
-  hprove (n2h_formula A ⟶ n2h_sequent l B) -> hprove (n2h_sequent l (imp A B)).
+  hprove (n2h_formula A → n2h_sequent l B) -> hprove (n2h_sequent l (imp A B)).
 Proof.
 induction l; simpl; intros A B pi; auto.
 apply IHl in pi.
@@ -383,8 +179,8 @@ eapply hprove_MP; [ eapply hprove_MP; [ apply hprove_Bsequent | ] | apply pi ]; 
 apply hprove_C.
 Qed.
 
-Lemma hprove_FRLsequent : forall x l A, ~ In x (flat_map (fun C => hffreevars (n2h_formula C)) l) ->
-  hprove ((hfrl x (n2h_sequent l A)) ⟶ n2h_sequent l (frl x A)).
+Lemma hprove_FRLsequent : forall x l A, ~ In x (flat_map (fun C => freevars (n2h_formula C)) l) ->
+  hprove ((frl x (n2h_sequent l A)) → n2h_sequent l (frl x A)).
 Proof.
 induction l; simpl; intros A Hf.
 - apply hprove_I.
@@ -398,104 +194,102 @@ Qed.
 End Fixed_r.
 
 
+Notation n2h_term := tesubs.
+Notation n2h_formula := esubs.
 Notation n2h_sequent r l A := (n2h_formula r (s2f l A)).
-Notation rgood_for r := (lgood_for r nil).
+Notation no_ecapture r := (no_ecapture_at r nil).
 
-Definition rsubs x y (r : nat -> hterm) n := htsubs x (hvar y) (r n).
+Definition rrename x y (r : nat -> hterm) n := tsubs x (tvar y) (r n).
 
-Lemma hfreevars_rsubs : forall x y r n z,
-  In z (hfreevars (rsubs x y r n)) -> (z = y /\ In x (hfreevars (r n))) \/ (In z (hfreevars (r n)) /\ z <> x).
-Proof. unfold rsubs; intros x y r n z Hin; apply hfreevars_tsubs in Hin; simpl in Hin; in_solve. Qed.
+Lemma tvars_rrename : forall x y r n z,
+  In z (tvars (rrename x y r n)) ->
+    (z = y /\ In x (tvars (r n))) \/ (In z (tvars (r n)) /\ z <> x).
+Proof. unfold rrename; intros x y r n z Hin; apply tvars_tsubs in Hin; simpl in Hin; in_solve. Qed.
 
-Lemma hfreevars_n2h_rsubs : forall x y r t z,
-  In z (hfreevars (n2h_term (rsubs x y r) t)) -> z = y \/ In z (hfreevars (n2h_term r t)).
-Proof. term_induction t; intros z Hin.
-- apply hfreevars_rsubs in Hin; intuition.
-- rewrite <- flat_map_concat_map in Hin.
-  apply in_flat_map in Hin; destruct Hin as [u [Huin Hinu]].
+Lemma tvars_n2h_rrename : forall x y r t z,
+  In z (tvars (n2h_term (rrename x y r) t)) -> z = y \/ In z (tvars (n2h_term r t)).
+Proof. term_induction t.
+- intros z Hin.
+  apply tvars_rrename in Hin; intuition.
+- rewrite flat_map_map in H.
+  apply in_flat_map in H; destruct H as [ u [Huin Hinu] ].
   specialize_Forall IHl with u; apply IHl in Hinu.
   destruct Hinu as [Hinu|Hinu]; [left; assumption | right].
   rewrite <- flat_map_concat_map; apply in_flat_map; exists u; intuition.
 Qed.
 
-Lemma hfreevars_n2h_rsubs_self : forall x y r t lv,
-  In x lv -> ltgood_for r lv t -> ~ In y (freevars t) ->
-  In y (hfreevars (n2h_term (rsubs x y r) t)) -> In y (hfreevars (n2h_term r t)).
-Proof. term_induction t; intros lv Hlv Hg Hnin Hin.
-- apply hfreevars_rsubs in Hin; destruct Hin as [Hin|Hin]; intuition.
-  specialize_Forall Hg with x; intuition.
-- apply Forall_fold_right in Hg.
-  apply in_flat_map in Hin; destruct Hin as [u [Huin Hinu]].
-  apply in_map_iff in Huin; destruct Huin as [v [Heq Hv]]; subst.
-  specialize_Forall_all v; apply IHl in Hg; intuition.
-  + rewrite <- flat_map_concat_map; apply in_flat_map; exists v; intuition.
-  + apply Hnin.
-    rewrite <- flat_map_concat_map; apply in_flat_map; exists v; intuition.
+Lemma tvars_n2h_rrename_self : forall x y r t,
+  no_tecapture_at r (x::nil) t -> ~ In y (tvars t) ->
+  In y (tvars (n2h_term (rrename x y r) t)) -> In y (tvars (n2h_term r t)).
+Proof. term_induction t.
+- intros Hg Hnin Hin.
+  apply tvars_rrename in Hin; destruct Hin as [Hin|Hin]; intuition.
+  inversion_clear Hg; intuition.
+- apply Forall_fold_right in H.
+  rewrite flat_map_map in H1; apply in_flat_map in H1; destruct H1 as [ u [Huin Hinu] ].
+  specialize_Forall_all u; apply IHl in H; intuition.
+  + rewrite <- flat_map_concat_map; apply in_flat_map; exists u; intuition.
+  + apply H0, in_flat_map; exists u; intuition.
 Qed.
 
-Lemma hffreevars_n2h_rsubs_self : forall x y r A lv,
-  In x lv -> lgood_for r lv A -> ~ In y (ffreevars A) ->
-  In y (hffreevars (n2h_formula (rsubs x y r) A)) -> In y (hffreevars (n2h_formula r A)).
+Lemma freevars_n2h_rrename_self : forall x y r (A : formula),
+  r #[[x::nil]] A -> ~ y ∈ A ->
+  y ∈ (n2h_formula (rrename x y r) A) -> y ∈ (n2h_formula r A).
 Proof. formula_induction A.
-- apply Forall_fold_right in H0.
-  apply in_flat_map in H2; destruct H2 as [u [Huin Hinu]].
-  apply in_map_iff in Huin; destruct Huin as [v [Heq Hv]]; subst.
-  specialize_Forall_all v.
-  apply hfreevars_n2h_rsubs_self with (lv:= lv) in Hinu; intuition.
-  + rewrite map_map, <- flat_map_concat_map; apply in_flat_map; exists v; intuition.
-  + apply H1.
-    apply in_flat_map; exists v; intuition.
-- apply in_or_app; apply in_app_or in H2; destruct H2 as [Hin|Hin]; [left|right].
-  + apply IHA1 with lv in Hin; intuition.
-  + apply IHA2 with lv in Hin; intuition.
-- refine ?[mygoal]. Existential 1 := ?mygoal.
-  apply in_remove in H2; destruct H2 as [Hin Hneq]; apply notin_remove; intuition.
-  apply IHA with lv; intuition.
-  + rewrite <- (app_nil_l _) in H0; now apply lgood_for_less in H0.
-  + apply H1; apply notin_remove; intuition.
+- apply Forall_fold_right in H.
+  rewrite flat_map_map in H1; apply in_flat_map in H1; destruct H1 as [ u [Huin Hinu] ].
+  specialize_Forall_all u.
+  apply tvars_n2h_rrename_self in Hinu; intuition.
+  + rewrite map_map, <- flat_map_concat_map; apply in_flat_map; exists u; intuition.
+  + apply H0, in_flat_map; exists u; intuition.
+- apply in_or_app; apply in_app_or in H1; destruct H1 as [Hin|Hin]; [left|right]; intuition.
+- apply in_remove in H1; destruct H1 as [Hin Hneq]; apply notin_remove; intuition.
+  apply IHA; intuition.
+  + apply no_ecapture_less with (lv1:= x::nil) in H; [ intuition | in_solve ].
+  + apply H0, notin_remove; intuition.
 Qed.
 
-Lemma hallvars_n2h_rsubs : forall x y r A z,
-  In z (hallvars (n2h_formula (rsubs x y r) A)) -> z = y \/ In z (hallvars (n2h_formula r A)).
+Lemma fvars_n2h_rrename : forall x y r (A : formula) z,
+  In z (fvars (n2h_formula (rrename x y r) A)) -> z = y \/ In z (fvars (n2h_formula r A)).
 Proof. formula_induction A.
-- apply in_flat_map in H; destruct H as [u [Huin Hinu]].
-  rewrite map_map in Huin.
-  apply in_map_iff in Huin; destruct Huin as [v [Heq Hv]]; subst.
-  apply hfreevars_n2h_rsubs in Hinu.
+- rewrite flat_map_map in H.
+  apply in_flat_map in H; destruct H as [ u [Huin Hinu] ].
+  apply tvars_n2h_rrename in Hinu.
   destruct Hinu as [Hinu|Hinu]; [left; intuition | right].
-  rewrite map_map, <- flat_map_concat_map; apply in_flat_map; exists v; intuition.
+  rewrite map_map, <- flat_map_concat_map; apply in_flat_map; exists u; intuition.
 - apply in_app_or in H; destruct H as [Hin|Hin].
   + apply IHA1 in Hin; intuition.
   + apply IHA2 in Hin; intuition.
-- refine ?[mygoal]. Existential 1 := ?mygoal.
-  intuition.
+- intuition.
   apply IHA in H0; intuition.
 Qed.
 
-Lemma tgood_for_fresh : forall r y x t lv, ~ In y (freevars t ++ lv) ->
-  ltgood_for r lv t -> ltgood_for (rsubs x y r) lv t.
+Lemma no_tecapture_rrename : forall r y x t lv, ~ In y (tvars t ++ lv) ->
+  no_tecapture_at r lv t -> no_tecapture_at (rrename x y r) lv t.
 Proof.
-term_induction t; intros lv Hin Hg.
-- apply Forall_forall; intros z Hz Hinz.
+term_induction t.
+- intros lv Hin Hg.
+  apply Forall_forall; intros z Hz Hinz.
   specialize_Forall Hg with z; apply Hg.
-  apply hfreevars_rsubs in Hinz; intuition; subst; intuition.
-- apply Forall_fold_right; apply Forall_fold_right in Hg.
+  apply tvars_rrename in Hinz; intuition; subst; intuition.
+- apply Forall_fold_right; apply Forall_fold_right in H0.
   apply Forall_forall; intros u Hu.
   specialize_Forall_all u.
   apply IHl; intuition.
-  apply in_map with (f:= freevars) in Hu.
-  apply Hin.
-  apply in_or_app; apply in_app_or in H; destruct H as [H|H]; [left|right]; intuition.
-  now apply in_flat_map; exists (freevars u).
+  apply in_map with (f:= tvars( T:=nat)) in Hu.
+  apply H.
+  apply in_or_app; apply in_app_or in H1; destruct H1 as [H1|H1]; [left|right]; intuition.
+  rewrite flat_map_concat_map.
+  now apply in_concat with (tvars u).
 Qed.
 
-Lemma good_for_fresh : forall r y x A lv, ~ In y (allvars A ++ lv) ->
-  lgood_for r lv A -> lgood_for (rsubs x y r) lv A.
+Lemma no_ecapture_rrename : forall r y x (A : formula) lv, ~ In y (fvars A ++ lv) ->
+  r #[[lv]] A -> (rrename x y r) #[[lv]] A.
 Proof. formula_induction A.
 - apply Forall_fold_right in H0; apply Forall_fold_right.
   apply Forall_forall; intros u Hu.
   specialize_Forall H0 with u.
-  apply tgood_for_fresh; intuition.
+  apply no_tecapture_rrename; intuition.
   apply H.
   apply in_or_app; apply in_app_or in H1; destruct H1 as [H1|H1]; [left|right]; intuition.
   now apply in_flat_map; exists u.
@@ -503,8 +297,6 @@ Proof. formula_induction A.
   apply H; in_solve.
 - apply IHA2; intuition.
   apply H; in_solve.
-- apply IHA; intuition.
-  apply in_app_or in H1; destruct H1 as [H1|H1]; try inversion H1; intuition; in_solve.
 - apply IHA; intuition.
   apply in_app_or in H1; destruct H1 as [H1|H1]; try inversion H1; intuition; in_solve.
 Qed.
@@ -517,476 +309,469 @@ Qed.
 Fixpoint rrefresh l ld r :=
 match l with
 | nil => r
-| x :: tl => let y := vfresh (l ++ ld) in rrefresh tl (x :: y :: ld) (rsubs x y r)
+| x :: tl => let y := fresh (l ++ ld) in rrefresh tl (x :: y :: ld) (rrename x y r)
 end.
 
-Lemma hfreevars_rrefresh : forall n l ld r z,
-  In z (l ++ ld) -> In z (hfreevars (rrefresh l ld r n)) -> In z (hfreevars (r n)).
+Lemma tvars_rrefresh : forall n l ld r z,
+  In z (l ++ ld) -> In z (tvars (rrefresh l ld r n)) -> In z (tvars (r n)).
 Proof.
 induction l; intros ld r z Hinz Hin; simpl in Hin; auto.
 apply IHl in Hin; intuition; try in_solve.
-apply hfreevars_rsubs in Hin; destruct Hin as [Hin|Hin]; intuition.
+apply tvars_rrename in Hin; destruct Hin as [Hin|Hin]; intuition.
 exfalso; subst.
-apply vfresh_prop with (a :: l ++ ld); in_solve.
+apply fresh_prop with (a :: l ++ ld); in_solve.
 Qed.
 
 Lemma rrefresh_notin : forall n z lvA lv r,
-  In z (hfreevars (rrefresh lvA lv r n)) -> ~ In z lvA.
+  In z (tvars (rrefresh lvA lv r n)) -> ~ In z lvA.
 Proof.
 induction lvA; simpl; intros lv r Hinf Hin; inversion Hin; subst; simpl in Hin.
-- apply hfreevars_rrefresh in Hinf; try in_solve.
-  apply hfreevars_rsubs in Hinf; destruct Hinf as [[Hinf _]|Hinf]; [ | intuition ].
-  apply vfresh_prop with (z :: lvA ++ lv); rewrite <- Hinf; now constructor.
+- apply tvars_rrefresh in Hinf; try in_solve.
+  apply tvars_rrename in Hinf; destruct Hinf as [ [Hinf _] | Hinf ]; [ | intuition ].
+  apply fresh_prop with (z :: lvA ++ lv); rewrite <- Hinf; now constructor.
 - now apply IHlvA in Hinf.
 Qed.
 
-Lemma good_for_refresh_preserv : forall l r ld lv A, incl (allvars A ++ lv) ld ->
-  lgood_for r lv A -> lgood_for (rrefresh l ld r) lv A.
+Lemma no_ecapture_rrefresh_preserv : forall l r ld lv (A : formula), incl (fvars A ++ lv) ld ->
+  r #[[lv]] A -> (rrefresh l ld r) #[[lv]] A.
 Proof.
 induction l; intros r ld lv A Hld Hg; simpl; auto.
 apply IHl; try (intros; in_solve).
-apply good_for_fresh; auto; intros Hin.
-apply vfresh_prop with (a :: l ++ ld).
+apply no_ecapture_rrename; auto; intros Hin.
+apply fresh_prop with (a :: l ++ ld).
 apply Hld in Hin; in_solve.
 Qed.
 
-Lemma tgood_for_refresh : forall ld t r lvt lv, incl (hfreevars (n2h_term r t) ++ lv) lvt ->
-  ltgood_for (rrefresh lvt ld r) lv t.
-Proof. term_induction t; intros r lvt lv Hincl.
-- apply Forall_forall; intros z Hz Hinz.
+Lemma no_tecapture_rrefresh : forall ld t r lvt lv, incl (tvars (n2h_term r t) ++ lv) lvt ->
+  no_tecapture_at (rrefresh lvt ld r) lv t.
+Proof. term_induction t.
+- intros r lvt lv Hincl.
+  apply Forall_forall; intros z Hz Hinz.
   apply rrefresh_notin in Hinz; apply Hinz; in_solve.
 - apply Forall_fold_right.
   apply Forall_forall; intros u Hu.
   specialize_Forall IHl with u; apply IHl.
-  intros z Hz; apply Hincl.
+  intros z Hz; apply H.
   apply in_or_app; apply in_app_or in Hz; destruct Hz as [Hz|Hz]; [left|right]; intuition.
-  apply in_map with (f:= fun x => hfreevars (n2h_term r x)) in Hu.
-  now rewrite flat_map_concat_map, map_map; apply in_flat_map; exists (hfreevars (n2h_term r u)).
+  apply in_map with (f:= fun x => tvars (n2h_term r x)) in Hu.
+  now rewrite flat_map_concat_map, map_map; apply in_flat_map; exists (tvars (n2h_term r u)).
 Qed.
 
-Lemma good_for_refresh : forall ld A r lvA lv, incl (hallvars (n2h_formula r A) ++ lv) lvA ->
-  lgood_for (rrefresh lvA ld r) lv A.
+Lemma no_ecapture_rrefresh : forall ld (A : formula) r lvA lv,
+  incl (fvars (n2h_formula r A) ++ lv) lvA -> (rrefresh lvA ld r) #[[lv]] A.
 Proof. formula_induction A; 
   (try apply IHA1); (try apply IHA2); (try apply IHA); try (intros z Hz; apply H; in_solve).
 apply Forall_fold_right.
 apply Forall_forall; intros u Hu.
-apply tgood_for_refresh.
+apply no_tecapture_rrefresh.
 intros z Hz; apply H.
 apply in_or_app; apply in_app_or in Hz; destruct Hz as [Hz|Hz]; [left|right]; intuition.
-apply in_map with (f:= fun x => hfreevars (n2h_term r x)) in Hu.
-rewrite map_map; apply in_flat_map; exists (hfreevars (n2h_term r u)); intuition.
+apply in_map with (f:= fun x => tvars (n2h_term r x)) in Hu.
+rewrite flat_map_concat_map, map_map; apply in_flat_map; exists (tvars (n2h_term r u)); intuition.
 Qed.
 
-Lemma bitsubs_fresh : forall r y x t,
-  ~ In y (freevars t ++ hfreevars (n2h_term r t)) ->
-  htsubs y (hvar x) (n2h_term (rsubs x y r) t) = n2h_term r t.
-Proof. term_induction t; intros Hnin.
-- now unfold rsubs; apply htbisubs.
-- f_equal.
-  apply map_ext_in; intros u Hinu.
-  specialize_Forall IHl with u; apply IHl; intros Hin; apply Hnin.
-  apply in_or_app; apply in_app_or in Hin; destruct Hin as [Hin|Hin]; [left|right].
-  + apply in_map with (f:= freevars) in Hinu; now apply in_flat_map; exists (freevars u).
-  + apply in_map with (f:= fun x => hfreevars (n2h_term r x)) in Hinu;
-      now apply in_flat_map; exists (hfreevars (n2h_term r u)).
+Lemma bitrename : forall r y x t,
+  ~ In y (tvars t ++ tvars (n2h_term r t)) ->
+  tsubs y (tvar x) (n2h_term (rrename x y r) t) = n2h_term r t.
+Proof. term_induction t.
+- intros Hnin.
+  now unfold rrename; apply notin_tsubs_bivar.
+- apply IHl; intros Hnin; apply H.
+  apply in_or_app; apply in_app_or in Hnin; destruct Hnin as [Hin|Hin]; [left|right].
+  + now apply in_flat_map; exists i.
+  + apply in_map with (f:= n2h_term r) in Hi.
+    now apply in_flat_map; exists (n2h_term r i).
 Qed.
 
-Lemma bisubs_fresh : forall r y x A,
-  ~ In y (allvars A ++ hffreevars (n2h_formula r A)) ->
-  hfsubs y (hvar x) (n2h_formula (rsubs x y r) A) = n2h_formula r A.
+Lemma birename : forall r y x (A : formula),
+  ~ In y (fvars A ++ freevars (n2h_formula r A)) ->
+  (n2h_formula (rrename x y r) A)[tvar x//y] = n2h_formula r A.
 Proof. formula_induction A.
-- apply bitsubs_fresh; intros Hin; apply H; in_solve.
+- apply bitrename; intros Hin; apply H; in_solve.
 - apply H; in_solve.
 - apply IHA1; intros Hin; apply H; in_solve.
 - apply IHA2; intros Hin; apply H; in_solve.
-- f_equal; case_analysis; intuition.
-  apply IHA; intros Hin; apply H1.
-  apply in_or_app; apply in_app_or in Hin; destruct Hin as [Hin|Hin]; [left|right]; intuition.
-  apply notin_remove; intuition.
-- f_equal; case_analysis; intuition.
-  apply IHA; intros Hin; apply H1.
+- apply IHA; intros Hin; apply H; right.
   apply in_or_app; apply in_app_or in Hin; destruct Hin as [Hin|Hin]; [left|right]; intuition.
   apply notin_remove; intuition.
 Qed.
 
-Lemma good_for_hilbert_rsubs : forall r y x A,
-  ~ In y (allvars A ++ hffreevars (n2h_formula r A)) -> rgood_for r A ->
-  hprove (n2h_formula (rsubs x y r) A) -> hprove (n2h_formula r A).
+Lemma hrrename : forall r y x (A : formula),
+  ~ In y (fvars A ++ freevars (n2h_formula r A)) -> no_ecapture r A ->
+  hprove (n2h_formula (rrename x y r) A) -> hprove (n2h_formula r A).
 Proof.
 intros r y x A Hnin Hg pi.
-rewrite <- bisubs_fresh with (x:=x) (y:=y); auto.
+rewrite <- birename with (x:=x) (y:=y); auto.
 eapply hprove_MP; [ apply hprove_INST | apply hprove_GEN ]; auto.
 simpl; repeat constructor.
-revert Hnin Hg; clear; induction A; simpl; intros; trivial.
+revert Hnin Hg; clear; formula_induction A.
+- apply IHA1; intuition; apply Hnin; in_solve.
+- apply IHA2; intuition; apply Hnin; in_solve.
 - split.
-  + apply IHA1; intuition; apply Hnin; in_solve.
-  + apply IHA2; intuition; apply Hnin; in_solve.
-- refine ?[mygoal]. Existential 1 := ?mygoal.
-  split.
   + apply IHA; intuition.
     * apply H2.
       apply in_or_app; apply in_app_or in H0; destruct H0 as [Hin|Hin]; [left|right]; intuition.
       apply notin_remove; intuition.
-    * rewrite <- (app_nil_l _) in Hg; apply lgood_for_less in Hg; auto.
+    * apply no_ecapture_less with (lv1:=nil) in Hg; [ intuition | in_solve ].
   + intros Heq; subst.
     apply Hnin; right.
     apply in_or_app; right.
     apply in_remove in H; destruct H as [Hin Hneq]; apply notin_remove; intuition.
-    apply hffreevars_n2h_rsubs_self with (lv:= c :: nil) in Hin; intuition.
+    apply freevars_n2h_rrename_self in Hin; intuition.
     apply H0, in_or_app; left.
-    now apply ffreevars_allvars.
+    now apply freevars_fvars.
 Qed.
 
-Lemma good_for_hilbert_rrefresh : forall l r ld A,
-  incl (hallvars (n2h_formula r A)) ld -> rgood_for r A ->
+Lemma hrrefresh : forall l r ld (A : formula),
+  incl (fvars (n2h_formula r A)) ld -> no_ecapture r A ->
   hprove (n2h_formula (rrefresh l ld r) A) -> hprove (n2h_formula r A).
 Proof.
 induction l; intros r ld A HA Hg pi; simpl; auto.
 apply IHl in pi.
-- apply good_for_hilbert_rsubs in pi; auto.
+- apply hrrename in pi; auto.
   intros Hin.
-  apply vfresh_prop with (a :: l ++ ld).
-  assert (Hincl := n2h_allvars r A).
+  apply fresh_prop with (a :: l ++ ld).
+  assert (Hincl := fvars_esubs r A).
   apply Hincl, HA in Hin; in_solve.
 - intros z Hz.
-  apply hallvars_n2h_rsubs in Hz; intuition; subst; intuition.
-- apply good_for_fresh; auto.
+  apply fvars_n2h_rrename in Hz; intuition; subst; intuition.
+- apply no_ecapture_rrename; auto.
   rewrite app_nil_r; intros Hin.
-  apply vfresh_prop with (a :: l ++ ld).
-  assert (Ha := n2h_allvars r A).
+  apply fresh_prop with (a :: l ++ ld).
+  assert (Ha := fvars_esubs r A).
   eapply or_introl in Hin; apply in_or_app, Ha, HA in Hin; in_solve.
 Qed.
 
 
-Definition rup t r n : hterm :=
-match n with
-| 0 => t
-| S k => r k
-end.
+Definition hfelift (u : hterm) r := fun n =>
+  match n with
+  | 0 => u
+  | S k => r k
+  end.
 
-Lemma tgood_for_rup : forall t r u lv,
-  ltgood_for r lv u -> ltgood_for (rup t r) lv (tup 0 u).
-Proof. term_induction u; intros lv HF.
-apply Forall_fold_right in HF; apply Forall_fold_right.
+Lemma no_tecapture_hfelift : forall u r t lv,
+  no_tecapture_at r lv t -> no_tecapture_at (hfelift u r) lv (tesubs ⇑ t).
+Proof. term_induction t.
+apply Forall_fold_right in H; apply Forall_fold_right.
 apply Forall_forall; intros z Hz.
-apply in_map_iff in Hz; destruct Hz as [y [Heq Hy]]; subst.
+apply in_map_iff in Hz; destruct Hz as [ y [Heq Hy] ]; subst.
 specialize_Forall_all y; auto.
 Qed.
 
-Lemma good_for_rup : forall t r A lv,
-  lgood_for r lv A -> lgood_for (rup t r) lv (fup 0 A).
+Lemma no_ecapture_hfelift : forall u r (A : formula) lv,
+  r #[[lv]] A -> (hfelift u r) #[[lv]] A↑.
 Proof. formula_induction A.
 apply Forall_fold_right in H; apply Forall_fold_right.
-apply Forall_forall; intros u Hu.
-apply in_map_iff in Hu; destruct Hu as [v [Heq Hv]]; subst.
-specialize_Forall H with v.
-now apply tgood_for_rup.
+apply Forall_forall; intros v Hv.
+apply in_map_iff in Hv; destruct Hv as [ v' [Heq Hv'] ]; subst.
+specialize_Forall H with v'.
+now apply no_tecapture_hfelift.
 Qed.
 
-Lemma good_for_rup_tsubs : forall r x y lv t,
-  ~ In y lv -> ~ In y (hfreevars (n2h_term r t)) ->
-  ltgood_for r lv t ->  ltgood_for (rup (hvar y) r) lv (tsubs x (dvar 0) (tup 0 t)).
-Proof. term_induction t; intros Hlv Hy Hg.
-- case_analysis; intuition.
+Lemma no_tecapture_hfeliftz : forall r x y lv t,
+  ~ In y lv -> ~ In y (tvars (n2h_term r t)) ->
+  no_tecapture_at r lv t -> no_tecapture_at (hfelift (tvar y) r) lv (tsubs x (dvar 0) (tesubs ⇑ t)).
+Proof. term_induction t.
+- intros Hlv Hy Hg.
+  case_analysis; intuition.
   apply Forall_forall; intros z Hz; intros Heqz; intuition; subst; intuition.
-- apply Forall_fold_right; apply Forall_fold_right in Hg.
+- apply Forall_fold_right; apply Forall_fold_right in H1.
   apply Forall_forall; intros z Hz.
-  apply in_map_iff in Hz; destruct Hz as [z' [Heq Hz]]; subst.
+  apply in_map_iff in Hz; destruct Hz as [ z' [Heq Hz] ]; subst.
   specialize_Forall_all z'.
   apply IHl; intuition.
-  apply Hy.
-  rewrite <- flat_map_concat_map; apply in_flat_map; exists z'; intuition.
+  apply H0.
+  rewrite flat_map_map; apply in_flat_map; exists z'; intuition.
 Qed.
 
-Lemma good_for_rup_subs : forall r x y A lv,
-  In x lv -> ~ In y lv -> ~ In y (hallvars (n2h_formula r A)) ->
-  lgood_for r lv A ->  lgood_for (rup (hvar y) r) lv (subs x (dvar 0) (fup 0 A)).
+Lemma no_ecapture_hfeliftz : forall r x y (A : formula) lv,
+  In x lv -> ~ In y lv -> ~ In y (fvars (n2h_formula r A)) ->
+  r #[[lv]] A -> (hfelift (tvar y) r) #[[lv]] A↑[dvar 0//x].
 Proof. formula_induction A;
 try rename H into Hxlv; try rename H0 into Hylv; try rename H1 into Hyl; try rename H2 into Hg.
 - apply Forall_fold_right in Hg; apply Forall_fold_right.
   rewrite map_map; apply Forall_forall; intros u Hu.
-  apply in_map_iff in Hu; destruct Hu as [v [Heq Hv]]; subst.
+  apply in_map_iff in Hu; destruct Hu as [ v [Heq Hv] ]; subst.
   specialize_Forall Hg with v.
-  apply good_for_rup_tsubs; intuition.
+  apply no_tecapture_hfeliftz; intuition.
   apply Hyl.
-  rewrite map_map, <- flat_map_concat_map; apply in_flat_map; exists v; intuition.
-- refine ?[mygoal]. Existential 1 := ?mygoal.
-  case_analysis.
-  + now apply good_for_rup.
-  + apply IHA; intuition.
-    apply Hylv.
-    destruct H as [Hin|Hin]; subst; intuition.
+  rewrite flat_map_map; apply in_flat_map; exists v; intuition.
+- now apply no_ecapture_hfelift.
+- apply IHA; intuition.
+  apply Hylv.
+  destruct H as [Hin|Hin]; subst; intuition.
 Qed.
 
-Lemma n2h_rup_term : forall t u r, n2h_term (rup t r) (tup 0 u) = n2h_term r u.
-Proof. term_induction u; intros r; f_equal.
-rewrite map_map; apply map_ext_in; intros v Hv.
-now specialize_Forall IHl with v.
-Qed.
+Lemma n2h_hfelift_tfup : forall t u r, n2h_term (hfelift t r) (tesubs ⇑ u) = n2h_term r u.
+Proof. term_induction u. Qed.
+Hint Resolve n2h_hfelift_tfup : term_db.
 
-Lemma n2h_rup : forall t A r, n2h_formula (rup t r) (fup 0 A) = n2h_formula r A.
-Proof. formula_induction A; apply n2h_rup_term. Qed.
+Lemma n2h_hfelift_fup : forall t (A : formula) r, n2h_formula (hfelift t r) A↑ = n2h_formula r A.
+Proof. formula_induction A. Qed.
 
-Lemma n2h_rup_subs : forall x lv t A r, In x lv -> lgood_for r lv A ->
-  n2h_formula (rup t r) (subs x (dvar 0) (fup 0 A)) = hfsubs x t (n2h_formula r A).
+Lemma n2h_hfelift_fupz : forall x t (A : formula) r, r #[[x::nil]] A ->
+  n2h_formula (hfelift t r) A↑[dvar 0//x] = (n2h_formula r A)[t//x].
 Proof.
-intros; rewrite n2h_subs with (lv:=lv); auto.
-- f_equal; apply n2h_rup.
-- now apply good_for_rup.
+intros; rewrite subs_esubs_no_ecapture.
+- f_equal; apply n2h_hfelift_fup.
+- now apply no_ecapture_hfelift.
 Qed.
 
 Proposition n2h : forall l A,
-  prove l A -> forall r, Forall (rgood_for r) (A :: l) -> hprove (n2h_sequent r l A).
+  prove l A -> forall r, Forall (no_ecapture r) (A :: l) -> hprove (n2h_sequent r l A).
 Proof.
 intros l A pi; induction pi; intros r Hg.
 - apply hprove_Ksequent, hprove_K2sequent.
 - apply IHpi.
   inversion_clear Hg as [ | ? ? Hg1 Hgl]; destruct Hg1; intuition.
-- assert ({rf : _ & Forall (rgood_for rf) (imp A B :: l)
+- assert ({rf : _ & Forall (no_ecapture rf) (imp A B :: l)
                   & hprove (n2h_sequent rf l B) -> hprove (n2h_sequent r l B)})
     as [rf Hg' Hp].
-  { exists (rrefresh (hallvars (n2h_formula r A))
-                     (flat_map (fun C => hallvars (n2h_formula r C)) (B :: l)) r).
+  { exists (rrefresh (fvars (n2h_formula r A))
+                     (flat_map (fun C => fvars (n2h_formula r C)) (B :: l)) r).
     - constructor; simpl; [split | ].
-      + apply good_for_refresh.
+      + apply no_ecapture_rrefresh.
         rewrite app_nil_r; apply incl_refl.
-      + apply good_for_refresh_preserv.
+      + apply no_ecapture_rrefresh_preserv.
         * rewrite app_nil_r; intros z Hz.
-          assert (Ha := n2h_allvars r B); in_solve.
+          assert (Ha := fvars_esubs r B); in_solve.
         * now inversion Hg.
       + apply Forall_forall; intros C HC.
-        apply good_for_refresh_preserv.
+        apply no_ecapture_rrefresh_preserv.
         * rewrite app_nil_r; intros z Hz.
-          assert (Ha := n2h_allvars r C).
+          assert (Ha := fvars_esubs r C).
           apply in_or_app; right.
           apply in_flat_map; exists C; intuition.
         * inversion Hg as [ | ? ? _ Hgl].
           now specialize_Forall Hgl with C.
-    - apply good_for_hilbert_rrefresh.
-      + apply n2h_sequent_allvars.
-      + now apply good_for_s2f. }
+    - apply hrrefresh.
+      + apply n2h_sequent_fvars.
+      + now apply no_ecapture_s2f. }
   apply Hp.
-  eapply hprove_MP; [ eapply hprove_MP; [ apply hprove_Ssequent | apply IHpi1 ] | apply IHpi2 ]; auto.
+  eapply hprove_MP;
+    [ eapply hprove_MP; [ apply hprove_Ssequent | apply IHpi1 ] | apply IHpi2 ]; auto.
   now inversion Hg' as [ | ? ? Hgi Hgl]; destruct Hgi; constructor.
-- remember (flat_map (fun C => hallvars (n2h_formula r C)) (frl x A :: l)) as lv.
-  remember (vfresh lv) as y.
-  remember (rup (hvar y) r) as r1.
+- remember (flat_map (fun C => fvars (n2h_formula r C)) (frl x A :: l)) as lv.
+  remember (fresh lv) as y.
+  remember (hfelift (tvar y) r) as r1.
   specialize IHpi with r1.
-  assert (Forall (rgood_for r1) (subs x (dvar 0) (fup 0 A) :: map (fup 0) l)) as pi'.
+  assert (Forall (no_ecapture r1) (A↑[dvar 0//x] :: map (esubs ⇑) l)) as pi'.
   { inversion_clear Hg as [ | ? ? Hgf Hgl ]; constructor.
-    - simpl in Hgf; apply good_for_rup_subs with (x:= x) (y:= y) in Hgf; intuition.
-      + rewrite <- (app_nil_l _) in Hgf; apply lgood_for_less in Hgf; now subst.
+    - simpl in Hgf; apply no_ecapture_hfeliftz with (x:= x) (y:= y) in Hgf; intuition.
+      + apply no_ecapture_less with (lv1:=nil) in Hgf; now subst.
       + simpl in H; destruct H; intuition; subst x.
-        apply vfresh_prop with lv; subst lv; in_solve.
-      + apply vfresh_prop with lv; rewrite <- Heqy; subst lv; in_solve.
+        apply fresh_prop with lv; subst lv; in_solve.
+      + apply fresh_prop with lv; rewrite <- Heqy; subst lv; in_solve.
     - apply Forall_forall; intros B HB.
-      apply in_map_iff in HB; destruct HB as [C [Heq HC]]; subst B.
+      apply in_map_iff in HB; destruct HB as [ C [Heq HC] ]; subst B.
       specialize_Forall Hgl with C.
-      now subst r1; apply good_for_rup. }
+      now subst r1; apply no_ecapture_hfelift. }
   apply IHpi in pi'.
   apply (hprove_GEN y) in pi'.
-  assert (hprove (n2h_sequent r1 (map (fup 0) l) (frl y (subs x (tvar y) (fup 0 A))))) as pi''.
+  assert (hprove (n2h_sequent r1 (map (esubs ⇑) l) (frl y (A↑[tvar y//x])))) as pi''.
   { eapply hprove_MP; [ apply hprove_FRLsequent | ].
     - intros Hin.
-      apply vfresh_prop with lv; rewrite <- Heqy; subst lv.
-      apply in_flat_map in Hin; destruct Hin as [C [HCin HinC]].
-      apply hffreevars_hallvars in HinC.
-      apply in_map_iff in HCin; destruct HCin as [D [Heq HD]]; subst C.
-      rewrite Heqr1, n2h_rup in HinC.
-      apply in_flat_map; exists D; in_solve.
-    - enough (n2h_sequent r1 (map (fup 0) l) (subs x (dvar 0) (fup 0 A))
-            = n2h_sequent r1 (map (fup 0) l) (subs x (tvar y) (fup 0 A))) as Heq
+      apply fresh_prop with lv; rewrite <- Heqy; subst lv.
+      rewrite flat_map_map in Hin; apply in_flat_map in Hin; destruct Hin as [ C [HCin HinC] ].
+      apply freevars_fvars in HinC.
+      rewrite Heqr1, n2h_hfelift_fup in HinC.
+      apply in_flat_map; exists C; in_solve.
+    - enough (n2h_sequent r1 (map (esubs ⇑) l) A↑[dvar 0//x]
+            = n2h_sequent r1 (map (esubs ⇑) l) A↑[tvar y//x]) as Heq
         by now rewrite <- Heq.
-      enough (n2h_formula r1 (subs x (dvar 0) (fup 0 A)) = n2h_formula r1 (subs x (tvar y) (fup 0 A))) as HeqBC.
-      { remember (subs x (dvar 0) (fup 0 A)) as B.
-        remember (subs x (tvar y) (fup 0 A)) as C.
+      enough (n2h_formula r1 A↑[dvar 0//x] = n2h_formula r1 A↑[tvar y//x]) as HeqBC.
+      { remember (A↑[dvar 0//x]) as B.
+        remember (A↑[tvar y//x]) as C.
         clear - HeqBC; revert B C HeqBC; induction l; simpl; intros B C HeqBC; intuition.
         apply IHl; simpl; f_equal; intuition. }
       subst r1; clear; formula_induction A; term_induction t. }
-  remember (frl y (subs x (tvar y) (fup 0 A))) as B.
+  remember (frl y A↑[tvar y//x]) as B.
   remember (frl x A) as C.
-  assert (hprove (n2h_formula r1 B ⟶ n2h_formula r C)) as pi'''.
+  assert (hprove (n2h_formula r1 B → n2h_formula r C)) as pi'''.
   { subst B C; clear - Hg Heqr1 Heqy Heqlv; simpl.
     eapply hprove_MP; [ apply hprove_FRL | ].
     - simpl; intros Hin.
       apply in_remove in Hin; destruct Hin as [Hin Hneq]; apply Hneq.
       inversion_clear Hg as [ | ? ? Hgx _ ]; simpl in Hgx.
-      apply good_for_rup with (t:= hvar y) in Hgx; rewrite <- Heqr1 in Hgx.
-      rewrite n2h_subs with (lv:= x :: nil) in Hin; intuition.
-      apply hffreevars_subs in Hin; simpl in Hin; intuition.
-    - assert (~ In y (hallvars (n2h_formula r1 (fup 0 A)))) as HA.
-      { intros Hin; rewrite Heqr1, n2h_rup in Hin.
-        apply vfresh_prop with lv; rewrite Heqlv at 2; rewrite <- Heqy; in_solve. }
+      apply no_ecapture_hfelift with (u:= tvar y) in Hgx; rewrite <- Heqr1 in Hgx.
+      rewrite subs_esubs_no_ecapture in Hin; intuition.
+      apply freevars_subs in Hin; simpl in Hin; intuition.
+    - assert (~ In y (fvars (n2h_formula r1 A↑))) as HA.
+      { intros Hin; rewrite Heqr1, n2h_hfelift_fup in Hin.
+        apply fresh_prop with lv; rewrite Heqlv at 2; rewrite <- Heqy; in_solve. }
       apply hprove_GEN.
-      eapply hprove_CUT; [ apply hprove_INST with (t:=hvar x) | ]; simpl.
+      eapply hprove_CUT; [ apply hprove_INST with (t:=tvar x) | ]; simpl.
       + repeat constructor.
         revert HA; clear; formula_induction A.
-        * refine ?[mygoal]. Existential 6 := ?mygoal.
-          revert H; case_analysis; intros Hin; [ | intuition ].
-          exfalso; apply HA.
-          apply in_remove in Hin; destruct Hin as [Hin _]; apply hffreevars_hallvars in Hin; intuition.
-      + enough (hfsubs y (hvar x) (n2h_formula r1 (subs x (tvar y) (fup 0 A))) = n2h_formula r A) as Heq
-          by (rewrite Heq; apply hprove_I).
-        rewrite n2h_subs with (lv:=x::nil); simpl; intuition; subst r1.
-        * rewrite hbisubs; intuition.
-          apply n2h_rup.
-        * apply good_for_rup.
+        revert H; case_analysis; intros Hin.
+        exfalso; apply HA.
+        apply in_remove in Hin; destruct Hin as [Hin _];
+          apply freevars_fvars in Hin; intuition.
+      + enough ((n2h_formula r1 (n2h_formula ⇑ A)[tvar y//x])[tvar x//y] = n2h_formula r A)
+          as Heq by (rewrite Heq; apply hprove_I).
+        rewrite subs_esubs_no_ecapture; simpl; intuition; subst r1.
+        * rewrite notin_subs_bivar; intuition.
+          apply n2h_hfelift_fup.
+        * apply no_ecapture_hfelift.
           now inversion Hg. }
   clear - Heqr1 pi'' pi'''.
   revert B C pi''' pi''; induction l; simpl; intros B C pBC pi.
   + eapply hprove_MP; eassumption.
-  + apply IHl with (imp (fup 0 a) B); intuition; simpl.
-    subst r1; rewrite n2h_rup.
+  + apply IHl with (imp a↑ B); intuition; simpl.
+    subst r1; rewrite n2h_hfelift_fup.
     eapply hprove_MP; [ apply hprove_B | apply pBC ].
-- assert ({rf : _ & Forall (rgood_for rf) (frl x A :: l) /\ rgood_for rf (subs x u A)
-                  & hprove (n2h_sequent rf l (subs x u A)) -> hprove (n2h_sequent r l (subs x u A))})
+- assert ({rf : _ & Forall (no_ecapture rf) (frl x A :: l) /\ no_ecapture rf (subs x u A)
+                  & hprove (n2h_sequent rf l A[u//x]) -> hprove (n2h_sequent r l A[u//x])})
     as [rf [Hg1 Hg2] Hp].
-  { exists (rrefresh (hallvars (n2h_formula r (frl x A)))
-                     (flat_map (fun C => hallvars (n2h_formula r C)) (subs x u A :: l)) r).
+  { exists (rrefresh (fvars (n2h_formula r (frl x A)))
+                     (flat_map (fun C => fvars (n2h_formula r C)) (subs x u A :: l)) r).
     - split; [ constructor; simpl | ].
-      + apply (good_for_refresh _ (frl x A) _ (hallvars (n2h_formula r (frl x A)))).
+      + apply (no_ecapture_rrefresh _ (frl x A) _ (fvars (n2h_formula r (frl x A)))).
         rewrite app_nil_r; now intros z Hz.
       + apply Forall_forall; intros C HC.
-        apply (good_for_refresh_preserv (hallvars (n2h_formula r (frl x A)))).
+        apply (no_ecapture_rrefresh_preserv (fvars (n2h_formula r (frl x A)))).
         * rewrite app_nil_r; intros z Hz; apply in_or_app; right.
           apply in_flat_map; exists C; intuition.
-          apply n2h_allvars; in_solve.
+          apply fvars_esubs; in_solve.
         * inversion_clear Hg as [ | ? ? _ Hgl ].
           now specialize_Forall Hgl with C.
-      + apply good_for_refresh_preserv.
+      + apply no_ecapture_rrefresh_preserv.
         * rewrite app_nil_r; intros z Hz; apply in_or_app; left.
-          apply n2h_allvars; in_solve.
+          apply fvars_esubs; in_solve.
         * now inversion Hg.
     - remember (subs x u A) as B.
-      apply good_for_hilbert_rrefresh.
-      + apply n2h_sequent_allvars.
-      + now apply good_for_s2f. }
+      apply hrrefresh.
+      + apply n2h_sequent_fvars.
+      + now apply no_ecapture_s2f. }
   apply Hp.
   eapply hprove_MP; [ eapply hprove_MP; [ apply hprove_Bsequent | ] | apply IHpi ]; auto.
-  rewrite n2h_subs with (lv:=x::nil); [ apply hprove_INST | | ]; intuition.
-  + apply lgood_hgood_closed with (lv := nil) (lv' := x :: nil); intuition.
+  rewrite subs_esubs_no_ecapture; [ apply hprove_INST | ]; intuition.
+  + apply no_ecapture_esubs_subs_closed; intuition.
     now inversion Hg1.
   + now inversion Hg1.
-- assert ({rf : _ & Forall (rgood_for rf) (exs x A :: l) /\ rgood_for rf (subs x u A)
+- assert ({rf : _ & Forall (no_ecapture rf) (exs x A :: l) /\ no_ecapture rf (subs x u A)
                   & hprove (n2h_sequent rf l (exs x A)) -> hprove (n2h_sequent r l (exs x A))})
     as [rf [Hg1 Hg2] Hp].
-  { exists (rrefresh (hallvars (n2h_formula r (subs x u A)))
-                     (flat_map (fun C => hallvars (n2h_formula r C)) (exs x A :: l)) r).
+  { exists (rrefresh (fvars (n2h_formula r (subs x u A)))
+                     (flat_map (fun C => fvars (n2h_formula r C)) (exs x A :: l)) r).
     - split; [ constructor; simpl | ].
-      + apply good_for_refresh_preserv.
+      + apply no_ecapture_rrefresh_preserv.
         * intros z Hz; apply in_app_or in Hz; destruct Hz as [Hz|Hz]; try in_solve.
-          eapply or_introl in Hz; apply in_or_app, n2h_allvars with (r:= r) in Hz; in_solve.
+          eapply or_introl in Hz; apply in_or_app, fvars_esubs with (r0:=r) in Hz; in_solve.
         * now inversion Hg.
       + apply Forall_forall; intros C HC.
-        apply (good_for_refresh_preserv (hallvars (n2h_formula r (subs x u A)))).
+        apply (no_ecapture_rrefresh_preserv (fvars (n2h_formula r (subs x u A)))).
         * rewrite app_nil_r; intros z Hz; right; apply in_or_app; right.
           apply in_flat_map; exists C; intuition.
-          apply n2h_allvars; in_solve.
+          apply fvars_esubs; in_solve.
         * inversion_clear Hg as [ | ? ? _ Hgl ].
           now specialize_Forall Hgl with C.
-      + apply (good_for_refresh _ (subs x u A) _ (hallvars (n2h_formula r (subs x u A)))).
+      + apply (no_ecapture_rrefresh _ (subs x u A) _ (fvars (n2h_formula r (subs x u A)))).
         rewrite app_nil_r; now intros z Hz.
     - remember (exs x A) as B.
-      apply good_for_hilbert_rrefresh.
-      + apply n2h_sequent_allvars.
-      + now apply good_for_s2f. }
+      apply hrrefresh.
+      + apply n2h_sequent_fvars.
+      + now apply no_ecapture_s2f. }
   apply Hp.
   eapply hprove_MP; [ eapply hprove_MP; [ apply hprove_Bsequent | ] | apply IHpi ]; auto.
-  + rewrite n2h_subs with (lv:=x::nil); simpl; [ apply hprove_EINST | | ]; intuition.
-    * apply lgood_hgood_closed with (lv := nil) (lv' := x :: nil); intuition.
+  + rewrite subs_esubs_no_ecapture; simpl; [ apply hprove_EINST | ]; intuition.
+    * apply no_ecapture_esubs_subs_closed; intuition.
       now inversion Hg1.
     * now inversion Hg1.
   + inversion Hg1; now constructor.
-- remember (rrefresh (hallvars (n2h_formula r (exs x A)))
-                     (flat_map (fun C => hallvars (n2h_formula r C)) (C :: l)) r) as r1.
-  assert (Forall (rgood_for r1) (C :: l)) as HgCl1.
+- remember (rrefresh (fvars (n2h_formula r (exs x A)))
+                     (flat_map (fun C => fvars (n2h_formula r C)) (C :: l)) r) as r1.
+  assert (Forall (no_ecapture r1) (C :: l)) as HgCl1.
   { apply Forall_forall; intros D HD.
     specialize_Forall Hg with D.
-    subst r1; apply good_for_refresh_preserv; intuition.
+    subst r1; apply no_ecapture_rrefresh_preserv; intuition.
     rewrite app_nil_r; intros z Hz.
     apply in_flat_map; exists D; intuition.
-    apply n2h_allvars; in_solve. }
-  assert (rgood_for r1 C) as HgC1 by (now inversion HgCl1).
-  assert (Forall (rgood_for r1) l) as Hgl1 by (now inversion HgCl1); clear HgCl1.
-  assert (rgood_for r1 (exs x A)) as HgA1
-    by (subst; apply good_for_refresh; rewrite app_nil_r; now intros z Hz).
-  apply good_for_hilbert_rrefresh with (l:=hallvars (n2h_formula r (exs x A)))
-                                       (ld:=flat_map (fun C => hallvars (n2h_formula r C)) (C :: l)).
-  + apply n2h_sequent_allvars.
-  + now apply good_for_s2f.
+    apply fvars_esubs; in_solve. }
+  assert (no_ecapture r1 C) as HgC1 by (now inversion HgCl1).
+  assert (Forall (no_ecapture r1) l) as Hgl1 by (now inversion HgCl1); clear HgCl1.
+  assert (no_ecapture r1 (exs x A)) as HgA1
+    by (subst; apply no_ecapture_rrefresh; rewrite app_nil_r; now intros z Hz).
+  apply hrrefresh with (l:=fvars (n2h_formula r (exs x A)))
+                       (ld:=flat_map (fun C => fvars (n2h_formula r C)) (C :: l)).
+  + apply n2h_sequent_fvars.
+  + now apply no_ecapture_s2f.
   + rewrite <- Heqr1.
-    eapply hprove_MP; [ eapply hprove_MP; [ apply hprove_Ssequent | ] | apply IHpi1; constructor; auto ].
+    eapply hprove_MP; [ eapply hprove_MP; [ apply hprove_Ssequent | ]
+                      | apply IHpi1; constructor; auto ].
     apply hprove_imp_sequent.
-    remember (flat_map (fun C => hallvars (n2h_formula r1 C)) (exs x A :: C :: l)) as lv.
-    remember (vfresh lv) as y.
-    assert (hprove (hexs x (n2h_formula r1 A) ⟶ hexs y (hfsubs x (hvar y) (n2h_formula r1 A)))) as pi'.
+    remember (flat_map (fun C => fvars (n2h_formula r1 C)) (exs x A :: C :: l)) as lv.
+    remember (fresh lv) as y.
+    assert (hprove (exs x (n2h_formula r1 A) → exs y (n2h_formula r1 A)[tvar y//x]))
+      as pi'.
     { remember (n2h_formula r1 A) as B; clear - HeqB Heqy Heqlv.
-      assert (~ In y (hallvars B)) as Hf
-        by (intros Hin; subst B; apply vfresh_prop with lv; rewrite Heqlv at 2; rewrite <- Heqy; in_solve).
+      assert (~ In y (fvars B)) as Hf
+        by (intros Hin; subst B; apply fresh_prop with lv; rewrite Heqlv at 2; rewrite <- Heqy;
+            in_solve).
       clear - Hf; eapply hprove_MP; [ apply hprove_EXS | ].
       - simpl; intros Hin; apply Hf.
         apply in_remove in Hin; destruct Hin as [Hin _].
-        apply hffreevars_subs in Hin; destruct Hin as [Hin|Hin]; intuition.
+        apply freevars_subs in Hin; destruct Hin as [Hin|Hin]; intuition.
         simpl in H; destruct H; intuition; subst.
-        now apply hffreevars_hallvars.
+        now apply freevars_fvars.
       - apply hprove_GEN.
-        replace (B ⟶ hexs y (hfsubs x (hvar y) B))
-           with (hfsubs y (hvar x) (hfsubs x (hvar y) B) ⟶ hexs y (hfsubs x (hvar y) B))
-          by now rewrite hbisubs.
+        replace (B → exs y B[tvar y//x])
+           with (B[tvar y//x][tvar x//y] → exs y B[tvar y//x])
+          by now rewrite notin_subs_bivar.
         apply hprove_EINST.
         simpl; repeat constructor.
         revert Hf; formula_induction B.
-        * refine ?[mygoal]. Existential 2 := ?mygoal.
-          revert H; case_analysis; intros Hin; apply in_remove in Hin; intuition.
-            -- exfalso; apply H2.
-               now apply hffreevars_hallvars.
-            -- apply H2.
-               now apply hffreevars_hallvars. }
+        revert H; case_analysis; intros Hin; apply in_remove in Hin; intuition.
+        * exfalso; apply H2.
+          now apply freevars_fvars.
+        * apply H2.
+          now apply freevars_fvars. }
     simpl; eapply hprove_CUT; [ apply pi' | ].
     eapply hprove_MP; [ apply hprove_EXS | ].
     * intros Hin.
-      apply vfresh_prop with lv; rewrite Heqlv at 2; rewrite <- Heqy.
+      apply fresh_prop with lv; rewrite Heqlv at 2; rewrite <- Heqy.
       simpl; right; apply in_or_app; right.
-      apply n2h_sequent_allvars, n2h_allvars; in_solve.
+      apply n2h_sequent_fvars, fvars_esubs; in_solve.
     * apply hprove_GEN.
-      replace (hvar y) with (n2h_term r1 (tvar y)) by reflexivity.
-      rewrite <- n2h_subs with (lv:=x::nil); auto; [ | now constructor ].
+      replace (tvar y) with (n2h_term r1 (tvar y)) by reflexivity.
+      rewrite <- subs_esubs_no_ecapture; auto.
       apply hprove_sequent_imp.
-      remember (rup (hvar y) r1) as r2.
-      assert (Forall (rgood_for r2) (fup 0 C :: subs x (dvar 0) (fup 0 A) :: map (fup 0) l)) as pi.
+      remember (hfelift (tvar y) r1) as r2.
+      assert (Forall (no_ecapture r2) (C↑ :: A↑[dvar 0//x] :: map (esubs ⇑) l)) as pi.
       { constructor; [ | constructor ]; subst r2.
-        - now apply good_for_rup.
-        - simpl in HgA1; apply good_for_rup_subs with (x:=x) (y:=y) in HgA1; intuition.
-          + rewrite <- (app_nil_l _) in HgA1; now apply lgood_for_less in HgA1.
+        - now apply no_ecapture_hfelift.
+        - simpl in HgA1; apply no_ecapture_hfeliftz with (x:=x) (y:=y) in HgA1; intuition.
+          + now apply no_ecapture_less with (lv1:=nil) in HgA1.
           + simpl in H; destruct H; intuition; subst x.
-            apply vfresh_prop with lv; rewrite Heqlv at 2; rewrite <- Heqy; now left.
-          + apply vfresh_prop with lv; rewrite Heqlv at 2; rewrite <- Heqy; in_solve.
+            apply fresh_prop with lv; rewrite Heqlv at 2; rewrite <- Heqy; now left.
+          + apply fresh_prop with lv; rewrite Heqlv at 2; rewrite <- Heqy; in_solve.
         - apply Forall_forall; intros E HE.
-          apply in_map_iff in HE; destruct HE as [E' [Heq HE]]; subst E.
+          apply in_map_iff in HE; destruct HE as [ E' [Heq HE] ]; subst E.
           specialize_Forall Hgl1 with E'.
-          now apply good_for_rup. }
+          now apply no_ecapture_hfelift. }
       apply IHpi2 in pi; simpl in pi.
-      remember (imp (subs x (dvar 0) (fup 0 A)) (fup 0 C)) as B.
-      remember (imp (subs x (tvar y) A) C) as D.
-      assert (hprove (n2h_formula r2 B ⟶ n2h_formula r1 D)) as HBD.
+      remember (A↑[dvar 0//x] → C↑) as B.
+      remember (A[tvar y//x] → C) as D.
+      assert (hprove (n2h_formula r2 B → n2h_formula r1 D)) as HBD.
       { subst B D r2; simpl; rewrite ? n2h_rup.
-        rewrite n2h_rup_subs with (lv:=x::nil); intuition.
-        enough (n2h_formula r1 (subs x (tvar y) A) = hfsubs x (hvar y) (n2h_formula r1 A))
+        rewrite n2h_hfelift_fupz; intuition.
+        rewrite n2h_hfelift_fup; intuition.
+        enough (n2h_formula r1 A[tvar y//x] = (n2h_formula r1 A)[tvar y//x])
           as Heq by (rewrite Heq; apply hprove_I).
-        apply n2h_subs with (x :: nil); intuition. }
+        rewrite subs_esubs_no_ecapture; intuition. }
       clear - Heqr2 pi HBD; revert B D pi HBD; induction l; simpl; intros B D pi HBD.
       -- eapply hprove_MP; eassumption.
-      -- apply IHl with (imp (fup 0 a) B); auto.
+      -- apply IHl with (a↑ → B); auto.
          simpl; subst.
-         rewrite n2h_rup.
+         rewrite n2h_hfelift_fup.
          eapply hprove_MP; [ apply hprove_B | apply HBD ].
 Qed.
 
-Proposition n2h_closed : forall r, (forall n, hclosed (r n)) ->
-  forall A, prove nil A -> hprove (n2h_formula r A).
+Proposition n2h_closed : forall r, fclosed r ->
+  forall A : formula, prove nil A -> hprove (n2h_formula r A).
 Proof.
 intros r Hc A pi; change (n2h_formula r A) with (n2h_sequent r nil A).
-now apply n2h; [ | apply Forall_forall; intros; apply lgood_for_closed ].
+now apply n2h; [ | apply Forall_forall; intros; apply fclosed_no_ecapture ].
 Qed.
 
 End N2H.
